Make RSL liveness proof work with Dafny 3.0.0

ironfleet/src/Dafny/Distributed/Common/Logic/Temporal/Temporal.s.dfy
@@ -24,49 +24,54 @@ predicate sat(s:int, t:temporal)
 }
 
 function{:opaque} and(x:temporal, y:temporal):temporal
-  ensures  forall i:int :: sat(i, and(x, y)) == (sat(i, x) && sat(i, y))
+  ensures  forall i:int {:trigger sat(i, and(x, y))} :: sat(i, and(x, y)) == (sat(i, x) && sat(i, y))
 {
   stepmap(imap i :: sat(i, x) && sat(i, y))
 }
 
 function{:opaque} or(x:temporal, y:temporal):temporal
-  ensures  forall i:int :: sat(i, or(x, y)) == (sat(i, x) || sat(i, y))
+  ensures  forall i:int {:trigger sat(i, or(x, y))} :: sat(i, or(x, y)) == (sat(i, x) || sat(i, y))
 {
   stepmap(imap i :: sat(i, x) || sat(i, y))
 }
 
 function{:opaque} imply(x:temporal, y:temporal):temporal
-  ensures  forall i:int :: sat(i, imply(x, y)) == (sat(i, x) ==> sat(i, y))
+  ensures  forall i:int {:trigger sat(i, imply(x, y))} :: sat(i, imply(x, y)) == (sat(i, x) ==> sat(i, y))
 {
   stepmap(imap i :: sat(i, x) ==> sat(i, y))
 }
 
 function{:opaque} equiv(x:temporal, y:temporal):temporal
-  ensures  forall i:int :: sat(i, equiv(x, y)) == (sat(i, x) <==> sat(i, y))
+  ensures  forall i:int {:trigger sat(i, equiv(x, y))} :: sat(i, equiv(x, y)) == (sat(i, x) <==> sat(i, y))
 {
   stepmap(imap i :: sat(i, x) <==> sat(i, y))
 }
 
 function{:opaque} not(x:temporal):temporal
-  ensures  forall i:int :: sat(i, not(x)) == !sat(i, x)
+  ensures  forall i:int {:trigger sat(i, not(x))} :: sat(i, not(x)) == !sat(i, x)
 {
   stepmap(imap i :: !sat(i, x))
 }
 
-function{:opaque} next(x:temporal):temporal
-  ensures  forall i:int {:trigger sat(i, next(x))} :: sat(i, next(x)) == sat(i+1, x)
+function nextstep(i:int):int
 {
-  stepmap(imap i :: sat(i+1, x))
+  i+1
+}
+
+function{:opaque} next(x:temporal):temporal
+  ensures  forall i:int {:trigger sat(i, next(x))} :: sat(i, next(x)) == sat(nextstep(i), x)
+{
+  stepmap(imap i :: sat(nextstep(i), x))
 }
 
 function{:opaque} always(x:temporal):temporal
 {
-  stepmap(imap i{:trigger sat(i, always(x))} :: forall j {:trigger sat(j, x)} :: i <= j ==> sat(j, x))
+  stepmap(imap i {:trigger sat(i, always(x))} :: forall j {:trigger sat(j, x)} :: i <= j ==> sat(j, x))
 }
 
 function{:opaque} eventual(x:temporal):temporal
 {
-  stepmap(imap i{:trigger sat(i, eventual(x))} :: exists j :: i <= j && sat(j, x))
+  stepmap(imap i {:trigger sat(i, eventual(x))} :: exists j :: i <= j && sat(j, x))
 }
 
 //}
