ironfleet/src/Dafny/Distributed/Protocol/RSL/LivenessProof/Assumptions.i.dfy
@@ -3,9 +3,21 @@ include "../CommonProof/Assumptions.i.dfy"
 include "../../../Common/Framework/EnvironmentSynchrony.s.dfy"
 
 module LivenessProof__Assumptions_i {
+import opened LiveRSL__Configuration_i
+import opened LiveRSL__Constants_i
 import opened LiveRSL__DistributedSystem_i
+import opened LiveRSL__Message_i
+import opened LiveRSL__Parameters_i
+import opened LiveRSL__Replica_i
+import opened LiveRSL__Types_i
 import opened CommonProof__Assumptions_i
 import opened EnvironmentSynchrony_s
+import opened Temporal__Temporal_s
+import opened Temporal__Time_s
+import opened Concrete_NodeIdentity_i
+import opened Collections__Maps2_s
+import opened Environment_s
+import opened Common__UpperBound_s
 
 ///////////////////////
 // TYPES
@@ -29,81 +41,81 @@ datatype AssumptionParameters = AssumptionParameters(
 
 function SetOfReplicaIndicesToSetOfHosts(s:set<int>, ids:seq<NodeIdentity>):set<NodeIdentity>
 {
-    set idx | idx in s && 0 <= idx < |ids| :: ids[idx]
+  set idx | idx in s && 0 <= idx < |ids| :: ids[idx]
 }
 
 predicate RslSchedulerActionOccursForReplica(
-    ps:RslState,
-    ps':RslState,
-    replica_index:int
-    )
+  ps:RslState,
+  ps':RslState,
+  replica_index:int
+  )
 {
-    exists ios {:trigger RslNextOneReplica(ps, ps', replica_index, ios)}
-           {:trigger LSchedulerNext(ps.replicas[replica_index], ps'.replicas[replica_index], ios) } ::
-       RslNextOneReplica(ps, ps', replica_index, ios)
+  exists ios {:trigger RslNextOneReplica(ps, ps', replica_index, ios)}
+        {:trigger LSchedulerNext(ps.replicas[replica_index], ps'.replicas[replica_index], ios) } ::
+    && RslNextOneReplica(ps, ps', replica_index, ios)
     && LSchedulerNext(ps.replicas[replica_index], ps'.replicas[replica_index], ios)
 }
 
 function{:opaque} MakeRslActionTemporalFromSchedulerFunction(
-    b:Behavior<RslState>,
-    replica_index:int
-    ):temporal
-    requires imaptotal(b);
-    ensures  forall i {:trigger sat(i, MakeRslActionTemporalFromSchedulerFunction(b, replica_index))} ::
-                 sat(i, MakeRslActionTemporalFromSchedulerFunction(b, replica_index)) <==>
-                 RslSchedulerActionOccursForReplica(b[i], b[i+1], replica_index);
+  b:Behavior<RslState>,
+  replica_index:int
+  ):temporal
+  requires imaptotal(b)
+  ensures  forall i {:trigger sat(i, MakeRslActionTemporalFromSchedulerFunction(b, replica_index))} ::
+               sat(i, MakeRslActionTemporalFromSchedulerFunction(b, replica_index)) <==>
+               RslSchedulerActionOccursForReplica(b[i], b[i+1], replica_index)
 {
-    stepmap(imap i :: RslSchedulerActionOccursForReplica(b[i], b[i+1], replica_index))
+  stepmap(imap i :: RslSchedulerActionOccursForReplica(b[i], b[i+1], replica_index))
 }
 
 function{:opaque} PaxosTimeMap(b:Behavior<RslState>):imap<int, int>
-    requires imaptotal(b);
-    ensures  imaptotal(PaxosTimeMap(b));
-    ensures  forall i {:trigger PaxosTimeMap(b)[i]} :: PaxosTimeMap(b)[i] == b[i].environment.time;
+  requires imaptotal(b)
+  ensures  imaptotal(PaxosTimeMap(b))
+  ensures  forall i {:trigger PaxosTimeMap(b)[i]} :: PaxosTimeMap(b)[i] == b[i].environment.time
 {
-    imap i :: b[i].environment.time
+  imap i :: b[i].environment.time
 }
 
 predicate ClientSendsRequestToReplica(ps:RslState, request:Request, replica:NodeIdentity)
-    requires request.Request?;
+  requires request.Request?
 {
-       ps.environment.nextStep.LEnvStepHostIos?
-    && ps.environment.nextStep.actor == request.client
-    && LIoOpSend(LPacket(replica, request.client, RslMessage_Request(request.seqno, request.request))) in ps.environment.nextStep.ios
+  && ps.environment.nextStep.LEnvStepHostIos?
+  && ps.environment.nextStep.actor == request.client
+  && LIoOpSend(LPacket(replica, request.client, RslMessage_Request(request.seqno, request.request))) in ps.environment.nextStep.ios
 }
 
 function{:opaque} ClientSendsRequestToReplicaTemporal(
-    b:Behavior<RslState>,
-    request:Request,
-    replica:NodeIdentity
-    ):temporal
-    requires imaptotal(b);
-    requires request.Request?;
-    ensures  forall i {:trigger sat(i, ClientSendsRequestToReplicaTemporal(b, request, replica))} ::
-                 sat(i, ClientSendsRequestToReplicaTemporal(b, request, replica)) <==>
-                 ClientSendsRequestToReplica(b[i], request, replica);
+  b:Behavior<RslState>,
+  request:Request,
+  replica:NodeIdentity
+  ):temporal
+  requires imaptotal(b)
+  requires request.Request?
+  ensures  forall i {:trigger sat(i, ClientSendsRequestToReplicaTemporal(b, request, replica))} ::
+               sat(i, ClientSendsRequestToReplicaTemporal(b, request, replica)) <==>
+               ClientSendsRequestToReplica(b[i], request, replica)
 {
-    stepmap(imap i :: ClientSendsRequestToReplica(b[i], request, replica))
+  stepmap(imap i :: ClientSendsRequestToReplica(b[i], request, replica))
 }
 
 predicate ClientNeverSentHigherSequenceNumberRequest(ps:RslState, request:Request)
-    requires request.Request?;
+  requires request.Request?
 {
-    forall p :: p in ps.environment.sentPackets && p.src == request.client && p.msg.RslMessage_Request? ==>
+  forall p :: p in ps.environment.sentPackets && p.src == request.client && p.msg.RslMessage_Request? ==>
         p.msg.seqno_req < request.seqno || (p.msg.seqno_req == request.seqno && p.msg.val == request.request)
 }
 
 function{:opaque} ClientNeverSentHigherSequenceNumberRequestTemporal(
-    b:Behavior<RslState>,
-    asp:AssumptionParameters
-    ):temporal
-    requires imaptotal(b);
-    requires asp.persistent_request.Request?;
-    ensures  forall i {:trigger sat(i, ClientNeverSentHigherSequenceNumberRequestTemporal(b, asp))} ::
-                 sat(i, ClientNeverSentHigherSequenceNumberRequestTemporal(b, asp)) <==>
-                 ClientNeverSentHigherSequenceNumberRequest(b[i], asp.persistent_request);
+  b:Behavior<RslState>,
+  asp:AssumptionParameters
+  ):temporal
+  requires imaptotal(b)
+  requires asp.persistent_request.Request?
+  ensures  forall i {:trigger sat(i, ClientNeverSentHigherSequenceNumberRequestTemporal(b, asp))} ::
+               sat(i, ClientNeverSentHigherSequenceNumberRequestTemporal(b, asp)) <==>
+               ClientNeverSentHigherSequenceNumberRequest(b[i], asp.persistent_request)
 {
-    stepmap(imap i :: ClientNeverSentHigherSequenceNumberRequest(b[i], asp.persistent_request))
+  stepmap(imap i :: ClientNeverSentHigherSequenceNumberRequest(b[i], asp.persistent_request))
 }
 
 ///////////////////////
@@ -111,73 +123,75 @@ function{:opaque} ClientNeverSentHigherSequenceNumberRequestTemporal(
 ///////////////////////
 
 predicate HostExecutesPeriodically(
-    b:Behavior<RslState>,
-    asp:AssumptionParameters,
-    replica_index:int
-    )
-    requires imaptotal(b);
+  b:Behavior<RslState>,
+  asp:AssumptionParameters,
+  replica_index:int
+  )
+  requires imaptotal(b)
 {
-    var scheduler_action := MakeRslActionTemporalFromSchedulerFunction(b, replica_index);
-    sat(asp.synchrony_start, always(eventuallynextwithin(scheduler_action, asp.host_period, PaxosTimeMap(b))))
+  var scheduler_action := MakeRslActionTemporalFromSchedulerFunction(b, replica_index);
+  sat(asp.synchrony_start, always(eventuallynextwithin(scheduler_action, asp.host_period, PaxosTimeMap(b))))
 }
 
 predicate PersistentClientSendsRequestPeriodically(
-    b:Behavior<RslState>,
-    asp:AssumptionParameters,
-    replica_index:int
-    )
-    requires imaptotal(b);
-    requires asp.persistent_request.Request?;
-    requires 0 <= replica_index < |asp.c.config.replica_ids|;
+  b:Behavior<RslState>,
+  asp:AssumptionParameters,
+  replica_index:int
+  )
+  requires imaptotal(b)
+  requires asp.persistent_request.Request?
+  requires 0 <= replica_index < |asp.c.config.replica_ids|
 {
-    var client_send := ClientSendsRequestToReplicaTemporal(b, asp.persistent_request, asp.c.config.replica_ids[replica_index]);
-    sat(asp.synchrony_start, always(eventuallynextwithin(client_send, asp.persistent_period, PaxosTimeMap(b))))
+  var client_send := ClientSendsRequestToReplicaTemporal(b, asp.persistent_request, asp.c.config.replica_ids[replica_index]);
+  sat(asp.synchrony_start, always(eventuallynextwithin(client_send, asp.persistent_period, PaxosTimeMap(b))))
 }
 
 predicate ReplyDeliveredDuringStep(ps:RslState, req:Request)
 {
-       req.Request?
-    && ps.environment.nextStep.LEnvStepDeliverPacket?
-    && var p := ps.environment.nextStep.p;
-          p.src in ps.constants.config.replica_ids
-       && p.dst == req.client
-       && p.msg.RslMessage_Reply?
-       && p.msg.seqno_reply == req.seqno
+  && req.Request?
+  && ps.environment.nextStep.LEnvStepDeliverPacket?
+  && var p := ps.environment.nextStep.p;
+    && p.src in ps.constants.config.replica_ids
+    && p.dst == req.client
+    && p.msg.RslMessage_Reply?
+    && p.msg.seqno_reply == req.seqno
 }
 
 function{:opaque} ReplyDeliveredTemporal(b:Behavior<RslState>, req:Request):temporal
-    requires imaptotal(b);
-    ensures forall i {:trigger sat(i, ReplyDeliveredTemporal(b, req))} ::
-                sat(i, ReplyDeliveredTemporal(b, req)) <==> ReplyDeliveredDuringStep(b[i], req);
+  requires imaptotal(b)
+  ensures forall i {:trigger sat(i, ReplyDeliveredTemporal(b, req))} ::
+              sat(i, ReplyDeliveredTemporal(b, req)) <==> ReplyDeliveredDuringStep(b[i], req)
 {
-    stepmap(imap i :: ReplyDeliveredDuringStep(b[i], req))
+  stepmap(imap i :: ReplyDeliveredDuringStep(b[i], req))
 }
 
 predicate OverflowProtectionNotUsedForReplica(ps:RslState, replica_index:int, params:LParameters, max_clock_ambiguity:int)
-    requires 0 <= replica_index < |ps.replicas|;
+  requires 0 <= replica_index < |ps.replicas|
 {
-    var s := ps.replicas[replica_index].replica;
-       LtUpperBound(s.proposer.election_state.current_view.seqno, params.max_integer_val)
-    && LeqUpperBound(ps.environment.time + max_clock_ambiguity + s.proposer.election_state.epoch_length, params.max_integer_val)
-    && LeqUpperBound(s.proposer.election_state.epoch_length + s.proposer.election_state.epoch_length, params.max_integer_val)
-    && LeqUpperBound(s.acceptor.log_truncation_point + params.max_log_length, params.max_integer_val)
-    && LtUpperBound(s.proposer.next_operation_number_to_propose, params.max_integer_val)
-    && LtUpperBound(s.executor.ops_complete, params.max_integer_val)
-    && LeqUpperBound(|s.proposer.election_state.requests_received_prev_epochs + s.proposer.election_state.requests_received_this_epoch|, params.max_integer_val)
-    && LtUpperBound(|s.proposer.election_state.requests_received_this_epoch|, params.max_integer_val)
+  var s := ps.replicas[replica_index].replica;
+  && LtUpperBound(s.proposer.election_state.current_view.seqno, params.max_integer_val)
+  && LeqUpperBound(ps.environment.time + max_clock_ambiguity + s.proposer.election_state.epoch_length, params.max_integer_val)
+  && LeqUpperBound(s.proposer.election_state.epoch_length + s.proposer.election_state.epoch_length, params.max_integer_val)
+  && LeqUpperBound(s.acceptor.log_truncation_point + params.max_log_length, params.max_integer_val)
+  && LtUpperBound(s.proposer.next_operation_number_to_propose, params.max_integer_val)
+  && LtUpperBound(s.executor.ops_complete, params.max_integer_val)
+  && LeqUpperBound(|s.proposer.election_state.requests_received_prev_epochs + s.proposer.election_state.requests_received_this_epoch|,
+                  params.max_integer_val)
+  && LtUpperBound(|s.proposer.election_state.requests_received_this_epoch|, params.max_integer_val)
 }
 
 predicate OverflowProtectionNotUsed(ps:RslState, params:LParameters, max_clock_ambiguity:int)
 {
-    forall replica_index :: 0 <= replica_index < |ps.replicas| ==> OverflowProtectionNotUsedForReplica(ps, replica_index, params, max_clock_ambiguity)
+  forall replica_index :: 0 <= replica_index < |ps.replicas| ==> OverflowProtectionNotUsedForReplica(ps, replica_index, params, max_clock_ambiguity)
 }
 
 function{:opaque} OverflowProtectionNotUsedTemporal(b:Behavior<RslState>, params:LParameters, max_clock_ambiguity:int):temporal
-    requires imaptotal(b);
-    ensures  forall i {:trigger sat(i, OverflowProtectionNotUsedTemporal(b, params, max_clock_ambiguity))} ::
-             sat(i, OverflowProtectionNotUsedTemporal(b, params, max_clock_ambiguity)) <==> OverflowProtectionNotUsed(b[i], params, max_clock_ambiguity);
+  requires imaptotal(b)
+  ensures  forall i {:trigger sat(i, OverflowProtectionNotUsedTemporal(b, params, max_clock_ambiguity))} ::
+           sat(i, OverflowProtectionNotUsedTemporal(b, params, max_clock_ambiguity))
+           <==> OverflowProtectionNotUsed(b[i], params, max_clock_ambiguity)
 {
-    stepmap(imap i :: OverflowProtectionNotUsed(b[i], params, max_clock_ambiguity))
+  stepmap(imap i :: OverflowProtectionNotUsed(b[i], params, max_clock_ambiguity))
 }
 
 ///////////////////////////
@@ -185,14 +199,14 @@ function{:opaque} OverflowProtectionNotUsedTemporal(b:Behavior<RslState>, params
 ///////////////////////////
 
 predicate LivenessAssumptions(
-    b:Behavior<RslState>,
-    asp:AssumptionParameters
-    )
+  b:Behavior<RslState>,
+  asp:AssumptionParameters
+  )
 {
-       IsValidBehavior(b, asp.c)
-    && var eb := RestrictBehaviorToEnvironment(b);
-       var live_hosts := SetOfReplicaIndicesToSetOfHosts(asp.live_quorum, asp.c.config.replica_ids);
-       HostQueuesLive(eb)
+  && IsValidBehavior(b, asp.c)
+  && var eb := RestrictBehaviorToEnvironment(b);
+    var live_hosts := SetOfReplicaIndicesToSetOfHosts(asp.live_quorum, asp.c.config.replica_ids);
+    && HostQueuesLive(eb)
 
     // The synchrony period start time is valid
     && 0 <= asp.synchrony_start
@@ -213,12 +227,14 @@ predicate LivenessAssumptions(
 
     // Each host in the live quorum executes periodically, with period asp.host_period
     && 0 < asp.host_period
-    && (forall replica_index {:trigger HostExecutesPeriodically(b, asp, replica_index)} :: replica_index in asp.live_quorum ==> HostExecutesPeriodically(b, asp, replica_index))
+    && (forall replica_index {:trigger HostExecutesPeriodically(b, asp, replica_index)} ::
+         replica_index in asp.live_quorum ==> HostExecutesPeriodically(b, asp, replica_index))
 
     // The persistent client sends its request periodically, with period asp.persistent_period
     && 0 < asp.persistent_period
     && asp.persistent_request.Request?
-    && (forall replica_index {:trigger PersistentClientSendsRequestPeriodically(b, asp, replica_index)} :: replica_index in asp.live_quorum ==> PersistentClientSendsRequestPeriodically(b, asp, replica_index))
+    && (forall replica_index {:trigger PersistentClientSendsRequestPeriodically(b, asp, replica_index)} ::
+         replica_index in asp.live_quorum ==> PersistentClientSendsRequestPeriodically(b, asp, replica_index))
 
     // and the persistent client never sends a request with a higher sequence number
     && sat(0, always(ClientNeverSentHigherSequenceNumberRequestTemporal(b, asp)))
