ironfleet/src/Dafny/Distributed/Protocol/RSL/LivenessProof/Execution.i.dfy
@@ -6,119 +6,133 @@ include "../CommonProof/Actions.i.dfy"
 
 module LivenessProof__Execution_i {
 
+import opened LiveRSL__Constants_i
+import opened LiveRSL__Configuration_i
 import opened LiveRSL__DistributedSystem_i
+import opened LiveRSL__Environment_i
+import opened LiveRSL__Executor_i
+import opened LiveRSL__Replica_i
+import opened LiveRSL__StateMachine_i
 import opened LivenessProof__Assumptions_i
 import opened LivenessProof__Invariants_i
 import opened LivenessProof__Environment_i
 import opened CommonProof__Actions_i
+import opened CommonProof__Constants_i
+import opened Concrete_NodeIdentity_i
+import opened Temporal__Temporal_s
+import opened Temporal__Rules_i
+import opened Environment_s
+import opened EnvironmentSynchrony_s
+import opened Collections__Maps2_s
+import opened Common__UpperBound_s
 
 predicate ReplySentToClientWithSeqno(ps:RslState, ps':RslState, client:NodeIdentity, seqno:int, idx:int, ios:seq<RslIo>, batch_idx:int)
 {
-       0 <= idx < |ps.replicas|
-    && 0 <= idx < |ps'.replicas|
-    && var s := ps.replicas[idx].replica;
-       var s' := ps'.replicas[idx].replica;
-          RslNextOneReplica(ps, ps', idx, ios)
-       && LReplicaNextSpontaneousMaybeExecute(s, s', ExtractSentPacketsFromIos(ios))
-       && s.executor.next_op_to_execute.OutstandingOpKnown?
-       && LtUpperBound(s.executor.ops_complete, s.executor.constants.all.params.max_integer_val)
-       && LReplicaConstantsValid(s.executor.constants)
-       && 0 <= batch_idx < |s.executor.next_op_to_execute.v|
-       && s.executor.next_op_to_execute.v[batch_idx].Request?
-       && s.executor.next_op_to_execute.v[batch_idx].client == client
-       && s.executor.next_op_to_execute.v[batch_idx].seqno == seqno
+  && 0 <= idx < |ps.replicas|
+  && 0 <= idx < |ps'.replicas|
+  && var s := ps.replicas[idx].replica;
+     var s' := ps'.replicas[idx].replica;
+     && RslNextOneReplica(ps, ps', idx, ios)
+     && LReplicaNextSpontaneousMaybeExecute(s, s', ExtractSentPacketsFromIos(ios))
+     && s.executor.next_op_to_execute.OutstandingOpKnown?
+     && LtUpperBound(s.executor.ops_complete, s.executor.constants.all.params.max_integer_val)
+     && LReplicaConstantsValid(s.executor.constants)
+     && 0 <= batch_idx < |s.executor.next_op_to_execute.v|
+     && s.executor.next_op_to_execute.v[batch_idx].Request?
+     && s.executor.next_op_to_execute.v[batch_idx].client == client
+     && s.executor.next_op_to_execute.v[batch_idx].seqno == seqno
 }
 
 predicate RequestWithSeqnoExecuted(ps:RslState, ps':RslState, client:NodeIdentity, seqno:int, idx:int)
 {
-    exists ios, batch_idx :: ReplySentToClientWithSeqno(ps, ps', client, seqno, idx, ios, batch_idx)
+  exists ios, batch_idx :: ReplySentToClientWithSeqno(ps, ps', client, seqno, idx, ios, batch_idx)
 }
 
 function {:opaque} RequestWithSeqnoExecutedTemporal(b:Behavior<RslState>, client:NodeIdentity, seqno:int, idx:int):temporal
-    requires imaptotal(b);
-    ensures  forall i {:trigger sat(i, RequestWithSeqnoExecutedTemporal(b, client, seqno, idx))} ::
-             sat(i, RequestWithSeqnoExecutedTemporal(b, client, seqno, idx)) <==> RequestWithSeqnoExecuted(b[i], b[i+1], client, seqno, idx);
+  requires imaptotal(b)
+  ensures  forall i {:trigger sat(i, RequestWithSeqnoExecutedTemporal(b, client, seqno, idx))} ::
+             sat(i, RequestWithSeqnoExecutedTemporal(b, client, seqno, idx)) <==> RequestWithSeqnoExecuted(b[i], b[i+1], client, seqno, idx)
 {
-    stepmap(imap i :: RequestWithSeqnoExecuted(b[i], b[i+1], client, seqno, idx))
+  stepmap(imap i :: RequestWithSeqnoExecuted(b[i], b[i+1], client, seqno, idx))
 }
 
 predicate ReplySentToClientAtLeastSeqno(ps:RslState, ps':RslState, client:NodeIdentity, seqno:int, idx:int, ios:seq<RslIo>, batch_idx:int)
 {
-       0 <= idx < |ps.replicas|
-    && 0 <= idx < |ps'.replicas|
-    && var s := ps.replicas[idx].replica;
-       var s' := ps'.replicas[idx].replica;
-          RslNextOneReplica(ps, ps', idx, ios)
-       && LReplicaNextSpontaneousMaybeExecute(s, s', ExtractSentPacketsFromIos(ios))
-       && s.executor.next_op_to_execute.OutstandingOpKnown?
-       && LtUpperBound(s.executor.ops_complete, s.executor.constants.all.params.max_integer_val)
-       && LReplicaConstantsValid(s.executor.constants)
-       && 0 <= batch_idx < |s.executor.next_op_to_execute.v|
-       && s.executor.next_op_to_execute.v[batch_idx].Request?
-       && s.executor.next_op_to_execute.v[batch_idx].client == client
-       && s.executor.next_op_to_execute.v[batch_idx].seqno >= seqno
+  && 0 <= idx < |ps.replicas|
+  && 0 <= idx < |ps'.replicas|
+  && var s := ps.replicas[idx].replica;
+     var s' := ps'.replicas[idx].replica;
+     && RslNextOneReplica(ps, ps', idx, ios)
+     && LReplicaNextSpontaneousMaybeExecute(s, s', ExtractSentPacketsFromIos(ios))
+     && s.executor.next_op_to_execute.OutstandingOpKnown?
+     && LtUpperBound(s.executor.ops_complete, s.executor.constants.all.params.max_integer_val)
+     && LReplicaConstantsValid(s.executor.constants)
+     && 0 <= batch_idx < |s.executor.next_op_to_execute.v|
+     && s.executor.next_op_to_execute.v[batch_idx].Request?
+     && s.executor.next_op_to_execute.v[batch_idx].client == client
+     && s.executor.next_op_to_execute.v[batch_idx].seqno >= seqno
 }
 
 predicate RequestAtLeastSeqnoExecuted(ps:RslState, ps':RslState, client:NodeIdentity, seqno:int, idx:int)
 {
-    exists ios, batch_idx :: ReplySentToClientAtLeastSeqno(ps, ps', client, seqno, idx, ios, batch_idx)
+  exists ios, batch_idx :: ReplySentToClientAtLeastSeqno(ps, ps', client, seqno, idx, ios, batch_idx)
 }
 
 function {:opaque} RequestAtLeastSeqnoExecutedTemporal(b:Behavior<RslState>, client:NodeIdentity, seqno:int, idx:int):temporal
-    requires imaptotal(b);
-    ensures  forall i {:trigger sat(i, RequestAtLeastSeqnoExecutedTemporal(b, client, seqno, idx))} ::
-             sat(i, RequestAtLeastSeqnoExecutedTemporal(b, client, seqno, idx)) <==> RequestAtLeastSeqnoExecuted(b[i], b[i+1], client, seqno, idx);
+  requires imaptotal(b)
+  ensures  forall i {:trigger sat(i, RequestAtLeastSeqnoExecutedTemporal(b, client, seqno, idx))} ::
+             sat(i, RequestAtLeastSeqnoExecutedTemporal(b, client, seqno, idx)) <==> RequestAtLeastSeqnoExecuted(b[i], b[i+1], client, seqno, idx)
 {
-    stepmap(imap i :: RequestAtLeastSeqnoExecuted(b[i], b[i+1], client, seqno, idx))
+  stepmap(imap i :: RequestAtLeastSeqnoExecuted(b[i], b[i+1], client, seqno, idx))
 }
 
 
 lemma lemma_PersistentRequestNeverExecuted(
-    b:Behavior<RslState>,
-    asp:AssumptionParameters,
-    idx:int
-    )
-    requires LivenessAssumptions(b, asp);
-    requires idx in asp.live_quorum;
-    ensures  sat(asp.synchrony_start, always(not(RequestWithSeqnoExecutedTemporal(b, asp.persistent_request.client, asp.persistent_request.seqno, idx))));
+  b:Behavior<RslState>,
+  asp:AssumptionParameters,
+  idx:int
+  )
+  requires LivenessAssumptions(b, asp)
+  requires idx in asp.live_quorum
+  ensures  sat(asp.synchrony_start, always(not(RequestWithSeqnoExecutedTemporal(b, asp.persistent_request.client, asp.persistent_request.seqno, idx))))
 {
-    var client := asp.persistent_request.client;
-    var seqno := asp.persistent_request.seqno;
-    var t := RequestWithSeqnoExecutedTemporal(b, client, seqno, idx);
+  var client := asp.persistent_request.client;
+  var seqno := asp.persistent_request.seqno;
+  var t := RequestWithSeqnoExecutedTemporal(b, client, seqno, idx);
     
-    forall i | asp.synchrony_start <= i
-        ensures !sat(i, t);
+  forall i | asp.synchrony_start <= i
+    ensures !sat(i, t)
+  {
+    if sat(i, t)
     {
-        if sat(i, t)
-        {
-            lemma_ConstantsAllConsistent(b, asp.c, i);
+      lemma_ConstantsAllConsistent(b, asp.c, i);
 
-            var ps := b[i];
-            var ps' := b[i+1];
-            var s := ps.replicas[idx].replica.executor;
-            var ios, batch_idx :| ReplySentToClientWithSeqno(ps, ps', client, seqno, idx, ios, batch_idx);
-            var sent_packets := ExtractSentPacketsFromIos(ios);
-            assert LExecutorExecute(ps.replicas[idx].replica.executor, ps'.replicas[idx].replica.executor, sent_packets);
+      var ps := b[i];
+      var ps' := b[i+1];
+      var s := ps.replicas[idx].replica.executor;
+      var ios, batch_idx :| ReplySentToClientWithSeqno(ps, ps', client, seqno, idx, ios, batch_idx);
+      var sent_packets := ExtractSentPacketsFromIos(ios);
+      assert LExecutorExecute(ps.replicas[idx].replica.executor, ps'.replicas[idx].replica.executor, sent_packets);
 
-            var batch := s.next_op_to_execute.v;
-            var temp := HandleRequestBatch(s.app, batch);
-            var new_state := temp.0[|temp.0|-1];
-            var replies := temp.1;
+      var batch := s.next_op_to_execute.v;
+      var temp := HandleRequestBatch(s.app, batch);
+      var new_state := temp.0[|temp.0|-1];
+      var replies := temp.1;
 
-            var me := s.constants.all.config.replica_ids[s.constants.my_index];
-            lemma_SpecificPacketInGetPacketsFromReplies(me, batch, replies, sent_packets, batch_idx);
-            var p := sent_packets[batch_idx];
-            assert LIoOpSend(p) in ios;
+      var me := s.constants.all.config.replica_ids[s.constants.my_index];
+      lemma_SpecificPacketInGetPacketsFromReplies(me, batch, replies, sent_packets, batch_idx);
+      var p := sent_packets[batch_idx];
+      assert LIoOpSend(p) in ios;
 
-            var delivery_step := lemma_PacketSentEventuallyDelivered(b, asp, i, p);
-            lemma_ConstantsAllConsistent(b, asp.c, delivery_step);
-            assert ReplyDeliveredDuringStep(b[delivery_step], asp.persistent_request);
-            TemporalDeduceFromAlways(0, delivery_step, not(ReplyDeliveredTemporal(b, asp.persistent_request)));
-            assert false;
-        }
+      var delivery_step := lemma_PacketSentEventuallyDelivered(b, asp, i, p);
+      lemma_ConstantsAllConsistent(b, asp.c, delivery_step);
+      assert ReplyDeliveredDuringStep(b[delivery_step], asp.persistent_request);
+      TemporalDeduceFromAlways(0, delivery_step, not(ReplyDeliveredTemporal(b, asp.persistent_request)));
+      assert false;
     }
+  }
 
-    TemporalAlways(asp.synchrony_start, not(t));
+  TemporalAlways(asp.synchrony_start, not(t));
 }
     
 }
