ironfleet/src/Dafny/Distributed/Protocol/RSL/LivenessProof/PacketHandling.i.dfy
@@ -1,5 +1,5 @@
-include "RoundRobin.i.dfy"
 include "RealTime.i.dfy"
+include "RoundRobin.i.dfy"
 include "../CommonProof/Environment.i.dfy"
 include "../CommonProof/Actions.i.dfy"
 include "../../../Common/Logic/Temporal/Heuristics.i.dfy"
@@ -11,422 +11,447 @@ include "../../../../Libraries/Math/mul.i.dfy"
 include "../../../../Libraries/Math/mul_auto.i.dfy"
 
 module LivenessProof__PacketHandling_i {
+import opened LiveRSL__Configuration_i
+import opened LiveRSL__Constants_i
+import opened LiveRSL__DistributedSystem_i
+import opened LiveRSL__Environment_i
+import opened LiveRSL__Replica_i
+import opened LivenessProof__Assumptions_i
+import opened LivenessProof__Environment_i
+import opened LivenessProof__Invariants_i
 import opened LivenessProof__RoundRobin_i
 import opened LivenessProof__RealTime_i
-import opened CommonProof__Environment_i
 import opened CommonProof__Actions_i
+import opened CommonProof__Assumptions_i
+import opened CommonProof__Constants_i
+import opened CommonProof__Environment_i
 import opened Temporal__Heuristics_i
 import opened Temporal__Rules_i
 import opened Temporal__Time_i
 import opened Temporal__LeadsTo_i
 import opened Liveness__EnvironmentSynchronyLemmas_i
+import opened Liveness__HostQueueLemmas_i
 import opened Math__mul_i
 import opened Math__mul_auto_i
+import opened Math__mul_nonlinear_i
+import opened Temporal__Temporal_s
+import opened Temporal__Time_s
+import opened Collections__Maps2_s
+import opened Collections__Maps2_i
+import opened Environment_s
+import opened EnvironmentSynchrony_s
+import opened Concrete_NodeIdentity_i
 
 predicate AllPacketsProcessedWithin(
-    b:Behavior<RslState>,
-    i:int,
-    processing_period:int,
-    sources:set<NodeIdentity>,
-    destinations:set<NodeIdentity>
-    )
-    requires imaptotal(b);
+  b:Behavior<RslState>,
+  i:int,
+  processing_period:int,
+  sources:set<NodeIdentity>,
+  destinations:set<NodeIdentity>
+  )
+  requires imaptotal(b)
 {
-    forall p {:trigger PacketSentBetweenHosts(b[i].environment, p, sources, destinations)} ::
-        PacketSentBetweenHosts(b[i].environment, p, sources, destinations) ==>
-        sat(i, eventuallynextwithin(PacketProcessedTemporal(b, p), processing_period, PaxosTimeMap(b)))
+  forall p {:trigger PacketSentBetweenHosts(b[i].environment, p, sources, destinations)} ::
+      PacketSentBetweenHosts(b[i].environment, p, sources, destinations) ==>
+      sat(i, eventuallynextwithin(PacketProcessedTemporal(b, p), processing_period, PaxosTimeMap(b)))
 }
 
 function{:opaque} AllPacketsProcessedWithinTemporal(
-    b:Behavior<RslState>,
-    processing_period:int,
-    sources:set<NodeIdentity>,
-    destinations:set<NodeIdentity>
-    ):temporal
-    requires imaptotal(b);
-    ensures  forall i {:trigger sat(i, AllPacketsProcessedWithinTemporal(b, processing_period, sources, destinations))} ::
-        sat(i, AllPacketsProcessedWithinTemporal(b, processing_period, sources, destinations)) <==>
-        AllPacketsProcessedWithin(b, i, processing_period, sources, destinations);
+  b:Behavior<RslState>,
+  processing_period:int,
+  sources:set<NodeIdentity>,
+  destinations:set<NodeIdentity>
+  ):temporal
+  requires imaptotal(b)
+  ensures  forall i {:trigger sat(i, AllPacketsProcessedWithinTemporal(b, processing_period, sources, destinations))} ::
+             sat(i, AllPacketsProcessedWithinTemporal(b, processing_period, sources, destinations)) <==>
+             AllPacketsProcessedWithin(b, i, processing_period, sources, destinations)
 {
-    stepmap(imap i :: AllPacketsProcessedWithin(b, i, processing_period, sources, destinations))
+  stepmap(imap i :: AllPacketsProcessedWithin(b, i, processing_period, sources, destinations))
 }
 
 
 lemma lemma_LReplicaNextProcessPacketOnlyReceivesOnePacket(
-    s:LReplica,
-    s':LReplica,
-    p:RslPacket,
-    ios:seq<RslIo>
-    )
-    requires LReplicaNextProcessPacket(s, s', ios);
-    requires LIoOpReceive(p) in ios;
-    ensures  ios[0] == LIoOpReceive(p);
+  s:LReplica,
+  s':LReplica,
+  p:RslPacket,
+  ios:seq<RslIo>
+  )
+  requires LReplicaNextProcessPacket(s, s', ios)
+  requires LIoOpReceive(p) in ios
+  ensures  ios[0] == LIoOpReceive(p)
 {
-    Lemma_IfOpSeqIsCompatibleWithReductionAndFirstIsntReceiveThenNoneAreReceives(ios);
-    assert ios[0].LIoOpReceive?;
+  Lemma_IfOpSeqIsCompatibleWithReductionAndFirstIsntReceiveThenNoneAreReceives(ios);
+  assert ios[0].LIoOpReceive?;
 
-    forall i | 0 < i < |ios|
-        ensures !ios[i].LIoOpReceive?;
+  forall i | 0 < i < |ios|
+    ensures !ios[i].LIoOpReceive?
+  {
+    if ios[0].r.msg.RslMessage_Heartbeat?
     {
-        if ios[0].r.msg.RslMessage_Heartbeat?
-        {
-            if i == 1
-            {
-                assert ios[i].LIoOpReadClock?;
-            }
-            else
-            {
-                assert ios[i] in ios[2..];
-                assert ios[i].LIoOpSend?;
-            }
-       }
-       else
-       {
-            assert ios[i] in ios[1..];
-            assert ios[i].LIoOpSend?;
-       }
+      if i == 1
+      {
+        assert ios[i].LIoOpReadClock?;
+      }
+      else
+      {
+        assert ios[i] in ios[2..];
+        assert ios[i].LIoOpSend?;
+      }
     }
-    assert ios[0] == LIoOpReceive(p);
+    else
+    {
+      assert ios[i] in ios[1..];
+      assert ios[i].LIoOpSend?;
+    }
+  }
+  assert ios[0] == LIoOpReceive(p);
 }
 
 
 lemma lemma_PacketReceiveCausesPacketProcessing(
-    b:Behavior<RslState>,
-    asp:AssumptionParameters,
-    p:RslPacket,
-    i:int
-    )
-    requires LivenessAssumptions(b, asp);
-    requires 0 <= i;
-    requires p.dst in asp.c.config.replica_ids;
-    requires sat(i, PacketReceivedTemporal(RestrictBehaviorToEnvironment(b), p));
-    ensures  PacketProcessedDuringAction(b[i], p);
+  b:Behavior<RslState>,
+  asp:AssumptionParameters,
+  p:RslPacket,
+  i:int
+  )
+  requires LivenessAssumptions(b, asp)
+  requires 0 <= i
+  requires p.dst in asp.c.config.replica_ids
+  requires sat(i, PacketReceivedTemporal(RestrictBehaviorToEnvironment(b), p))
+  ensures  PacketProcessedDuringAction(b[i], p)
 {
-    var eb := RestrictBehaviorToEnvironment(b);
-    var ps := b[i];
-    var ps' := b[i+1];
+  var eb := RestrictBehaviorToEnvironment(b);
+  var ps := b[i];
+  var ps' := b[i+1];
 
-    lemma_AssumptionsMakeValidTransition(b, asp.c, i);
-    lemma_HostQueuesNext(b, asp, i);
-    lemma_ConstantsAllConsistent(b, asp.c, i);
+  lemma_AssumptionsMakeValidTransition(b, asp.c, i);
+  lemma_HostQueuesNext(b, asp, i);
+  lemma_ConstantsAllConsistent(b, asp.c, i);
 
-    assert sat(i, PacketReceivedTemporal(eb, p));
-    assert PacketReceivedDuringAction(ps.environment, p);
-    var ios := ps.environment.nextStep.ios;
-    var io := LIoOpReceive(p);
-    assert io in ios;
-    assert IsValidLIoOp(io, p.dst, ps.environment);
+  assert sat(i, PacketReceivedTemporal(eb, p));
+  assert PacketReceivedDuringAction(ps.environment, p);
+  var ios := ps.environment.nextStep.ios;
+  var io := LIoOpReceive(p);
+  assert io in ios;
+  assert IsValidLIoOp(io, p.dst, ps.environment);
 
-    Lemma_ReceiveMakesHostQueueSmaller(ps.environment.hostInfo[p.dst].queue, ps'.environment.hostInfo[p.dst].queue, ios, p);
-    assert ps'.environment.hostInfo[p.dst].queue != ps.environment.hostInfo[p.dst].queue;
+  Lemma_ReceiveMakesHostQueueSmaller(ps.environment.hostInfo[p.dst].queue, ps'.environment.hostInfo[p.dst].queue, ios, p);
+  assert ps'.environment.hostInfo[p.dst].queue != ps.environment.hostInfo[p.dst].queue;
 
-    if (exists idx, ios' :: RslNextOneReplica(ps, ps', idx, ios'))
-    {
-        var idx, ios' :| RslNextOneReplica(ps, ps', idx, ios');
-        Lemma_ReceiveRemovesPacketFromHostQueue(ps.environment.hostInfo[p.dst].queue, ps'.environment.hostInfo[p.dst].queue, ios, p);
-        Lemma_RemovePacketFromHostQueueImpliesReceive(ps.environment.hostInfo[p.dst].queue, ps'.environment.hostInfo[p.dst].queue, ios', p);
-        assert io in ios';
-        lemma_LReplicaNextProcessPacketOnlyReceivesOnePacket(ps.replicas[idx].replica, ps'.replicas[idx].replica, p, ios');
-        assert PacketProcessedViaIos(b[i], b[i+1], p, idx, ios');
-    }
-    else if (exists eid, ios' :: RslNextOneExternal(ps, ps', eid, ios'))
-    {
-        var eid, ios' :| RslNextOneExternal(ps, ps', eid, ios');
-        assert eid !in ps.constants.config.replica_ids;
-        assert p.dst != eid;
-        assert HostQueue_PerformIos(ps.environment.hostInfo[p.dst].queue, ps'.environment.hostInfo[p.dst].queue, []);
-        assert ps'.environment.hostInfo[p.dst] == ps.environment.hostInfo[p.dst];
-        assert false;
-    }
-    else
-    {
-        assert false;
-    }
+  if (exists idx, ios' :: RslNextOneReplica(ps, ps', idx, ios'))
+  {
+    var idx, ios' :| RslNextOneReplica(ps, ps', idx, ios');
+    Lemma_ReceiveRemovesPacketFromHostQueue(ps.environment.hostInfo[p.dst].queue, ps'.environment.hostInfo[p.dst].queue, ios, p);
+    Lemma_RemovePacketFromHostQueueImpliesReceive(ps.environment.hostInfo[p.dst].queue, ps'.environment.hostInfo[p.dst].queue, ios', p);
+    assert io in ios';
+    lemma_LReplicaNextProcessPacketOnlyReceivesOnePacket(ps.replicas[idx].replica, ps'.replicas[idx].replica, p, ios');
+    assert PacketProcessedViaIos(b[i], b[i+1], p, idx, ios');
+  }
+  else if (exists eid, ios' :: RslNextOneExternal(ps, ps', eid, ios'))
+  {
+    var eid, ios' :| RslNextOneExternal(ps, ps', eid, ios');
+    assert eid !in ps.constants.config.replica_ids;
+    assert p.dst != eid;
+    assert HostQueue_PerformIos(ps.environment.hostInfo[p.dst].queue, ps'.environment.hostInfo[p.dst].queue, []);
+    assert ps'.environment.hostInfo[p.dst] == ps.environment.hostInfo[p.dst];
+    assert false;
+  }
+  else
+  {
+    assert false;
+  }
 }
 
 
 lemma lemma_IfPacketsSynchronousForHostsThenSynchronousForFewerHosts<IdType, MessageType>(
-    b:Behavior<LEnvironment<IdType, MessageType>>,
-    sync_start:int,
-    latency_bound:int,
-    sources:set<IdType>,
-    destinations:set<IdType>,
-    sources':set<IdType>,
-    destinations':set<IdType>
-    )
-    requires imaptotal(b);
-    requires NetworkSynchronousForHosts(b, sync_start, latency_bound, sources, destinations);
-    requires sources' <= sources;
-    requires destinations' <= destinations;
-    ensures  NetworkSynchronousForHosts(b, sync_start, latency_bound, sources', destinations');
+  b:Behavior<LEnvironment<IdType, MessageType>>,
+  sync_start:int,
+  latency_bound:int,
+  sources:set<IdType>,
+  destinations:set<IdType>,
+  sources':set<IdType>,
+  destinations':set<IdType>
+  )
+  requires LEnvironment_BehaviorSatisfiesSpec(b)
+  requires NetworkSynchronousForHosts(b, sync_start, latency_bound, sources, destinations)
+  requires 0 <= sync_start
+  requires sources' <= sources
+  requires destinations' <= destinations
+  ensures  NetworkSynchronousForHosts(b, sync_start, latency_bound, sources', destinations')
 {
-    forall i | sync_start <= i
-        ensures sat(i, PacketsSynchronousForHostsTemporal(b, latency_bound, sources', destinations'));
+  forall i | sync_start <= i
+    ensures sat(i, PacketsSynchronousForHostsTemporal(b, latency_bound, sources', destinations'))
+  {
+    forall p | PacketSentBetweenHosts(b[i], p, sources', destinations')
+      ensures sat(i, next(eventuallynextwithin(PacketDeliveredTemporal(b, p), latency_bound, BehaviorToTimeMap(b))))
     {
-        forall p | PacketSentBetweenHosts(b[i], p, sources', destinations')
-            ensures sat(i, next(eventuallynextwithin(PacketDeliveredTemporal(b, p), latency_bound, BehaviorToTimeMap(b))));
-        {
-            assert PacketSentBetweenHosts(b[i], p, sources, destinations);
-            TemporalDeduceFromAlways(sync_start, i, PacketsSynchronousForHostsTemporal(b, latency_bound, sources, destinations));
-        }
+      assert PacketSentBetweenHosts(b[i], p, sources, destinations);
+      TemporalDeduceFromAlways(sync_start, i, PacketsSynchronousForHostsTemporal(b, latency_bound, sources, destinations));
+      lemma_PacketSentAppearsInSentPacketsEnvironment(b, i, p);
     }
-    TemporalAlways(sync_start, PacketsSynchronousForHostsTemporal(b, latency_bound, sources', destinations'));
+  }
+  TemporalAlways(sync_start, PacketsSynchronousForHostsTemporal(b, latency_bound, sources', destinations'));
 }
 
 lemma lemma_AllPacketsReceivedInTime(
-    b:Behavior<RslState>,
-    asp:AssumptionParameters
-    ) returns
-    (processing_sync_start:int,
-     processing_bound:int)
-    requires LivenessAssumptions(b, asp);
-    ensures  asp.synchrony_start <= processing_sync_start;
-    ensures  processing_bound == asp.latency_bound + asp.burst_size * TimeToPerformGenericAction(asp);
-    ensures  var eb := RestrictBehaviorToEnvironment(b);
-             var sources := SetOfReplicaIndicesToSetOfHosts(asp.live_quorum, asp.c.config.replica_ids) + {asp.persistent_request.client};
-             var destinations := SetOfReplicaIndicesToSetOfHosts(asp.live_quorum, asp.c.config.replica_ids);
-             sat(processing_sync_start, always(AllPacketsReceivedWithinTemporal(eb, processing_bound, sources, destinations)));
+  b:Behavior<RslState>,
+  asp:AssumptionParameters
+  ) returns (
+  processing_sync_start:int,
+  processing_bound:int
+  )
+  requires LivenessAssumptions(b, asp)
+  ensures  asp.synchrony_start <= processing_sync_start
+  ensures  processing_bound == asp.latency_bound + asp.burst_size * TimeToPerformGenericAction(asp)
+  ensures  var eb := RestrictBehaviorToEnvironment(b);
+           var sources := SetOfReplicaIndicesToSetOfHosts(asp.live_quorum, asp.c.config.replica_ids) + {asp.persistent_request.client};
+           var destinations := SetOfReplicaIndicesToSetOfHosts(asp.live_quorum, asp.c.config.replica_ids);
+           sat(processing_sync_start, always(AllPacketsReceivedWithinTemporal(eb, processing_bound, sources, destinations)))
 {
-    var eb := RestrictBehaviorToEnvironment(b);
-    var sources := SetOfReplicaIndicesToSetOfHosts(asp.live_quorum, asp.c.config.replica_ids) + {asp.persistent_request.client};
-    var destinations := SetOfReplicaIndicesToSetOfHosts(asp.live_quorum, asp.c.config.replica_ids);
-    var receive_period := TimeToPerformGenericAction(asp);
-    var burst_period := asp.burst_size * TimeToPerformGenericAction(asp) + 1;
-    var real_time_fun := PaxosTimeMap(b);
+  var eb := RestrictBehaviorToEnvironment(b);
+  var sources := SetOfReplicaIndicesToSetOfHosts(asp.live_quorum, asp.c.config.replica_ids) + {asp.persistent_request.client};
+  var destinations := SetOfReplicaIndicesToSetOfHosts(asp.live_quorum, asp.c.config.replica_ids);
+  var receive_period := TimeToPerformGenericAction(asp);
+  var burst_period := asp.burst_size * TimeToPerformGenericAction(asp) + 1;
+  var real_time_fun := PaxosTimeMap(b);
 
-    lemma_mul_is_associative(asp.burst_size, asp.host_period, LReplicaNumActions());
+  lemma_mul_is_associative(asp.burst_size, asp.host_period, LReplicaNumActions());
     
-    forall i {:trigger real_time_fun[i]} {:trigger BehaviorToTimeMap(eb)[i]}
-        ensures real_time_fun[i] == BehaviorToTimeMap(eb)[i];
-    {
-    }
-    assert real_time_fun == BehaviorToTimeMap(eb);
+  forall i {:trigger real_time_fun[i]} {:trigger BehaviorToTimeMap(eb)[i]}
+    ensures real_time_fun[i] == BehaviorToTimeMap(eb)[i]
+  {
+  }
+  assert real_time_fun == BehaviorToTimeMap(eb);
 
-    lemma_AssumptionsMakeValidEnvironmentBehavior(b, asp.c);
-    assert LEnvironment_BehaviorSatisfiesSpec(eb);
+  lemma_AssumptionsMakeValidEnvironmentBehavior(b, asp.c);
+  assert LEnvironment_BehaviorSatisfiesSpec(eb);
 
-    assert NetworkSynchronousForHosts(eb, asp.synchrony_start, asp.latency_bound, sources, sources);
-    lemma_IfPacketsSynchronousForHostsThenSynchronousForFewerHosts(eb, asp.synchrony_start, asp.latency_bound, sources, sources, sources, destinations);
-    assert NetworkSynchronousForHosts(eb, asp.synchrony_start, asp.latency_bound, sources, destinations);
-    assert sat(asp.synchrony_start, always(PacketsSynchronousForHostsTemporal(eb, asp.latency_bound, sources, destinations)));
-    TemporalEventually(0, asp.synchrony_start, always(PacketsSynchronousForHostsTemporal(eb, asp.latency_bound, sources, destinations)));
+  assert NetworkSynchronousForHosts(eb, asp.synchrony_start, asp.latency_bound, sources, sources);
+  lemma_IfPacketsSynchronousForHostsThenSynchronousForFewerHosts(eb, asp.synchrony_start, asp.latency_bound, sources,
+                                                                 sources, sources, destinations);
+  assert NetworkSynchronousForHosts(eb, asp.synchrony_start, asp.latency_bound, sources, destinations);
+  assert sat(asp.synchrony_start, always(PacketsSynchronousForHostsTemporal(eb, asp.latency_bound, sources, destinations)));
+  TemporalEventually(0, asp.synchrony_start, always(PacketsSynchronousForHostsTemporal(eb, asp.latency_bound, sources, destinations)));
 
-    forall host | host in destinations
-        ensures sat(0, eventual(always(NetworkDeliveryRateForHostBoundedTemporal(eb, asp.burst_size, burst_period, host))));
-    {
-        var replica_index :| replica_index in asp.live_quorum && host == asp.c.config.replica_ids[replica_index];
-        assert sat(asp.synchrony_start, always(NetworkDeliveryRateForHostBoundedTemporal(eb, asp.burst_size, burst_period, host)));
-        TemporalEventually(0, asp.synchrony_start, always(NetworkDeliveryRateForHostBoundedTemporal(eb, asp.burst_size, burst_period, host)));
-    }
+  forall host | host in destinations
+    ensures sat(0, eventual(always(NetworkDeliveryRateForHostBoundedTemporal(eb, asp.burst_size, burst_period, host))))
+  {
+    var replica_index :| replica_index in asp.live_quorum && host == asp.c.config.replica_ids[replica_index];
+    assert sat(asp.synchrony_start, always(NetworkDeliveryRateForHostBoundedTemporal(eb, asp.burst_size, burst_period, host)));
+    TemporalEventually(0, asp.synchrony_start, always(NetworkDeliveryRateForHostBoundedTemporal(eb, asp.burst_size, burst_period, host)));
+  }
     
-    lemma_mul_is_associative(asp.burst_size, asp.host_period, LReplicaNumActions());
-    assert forall host :: host in destinations ==> sat(0, eventual(always(NetworkDeliveryRateForHostBoundedTemporal(eb, asp.burst_size, asp.burst_size * receive_period + 1, host))));
+  lemma_mul_is_associative(asp.burst_size, asp.host_period, LReplicaNumActions());
+  assert forall host :: host in destinations ==> sat(0, eventual(always(NetworkDeliveryRateForHostBoundedTemporal(eb, asp.burst_size, asp.burst_size * receive_period + 1, host))));
 
-    forall host | host in destinations
-        ensures sat(asp.synchrony_start, always(eventuallynextwithin(ReceiveAttemptedTemporal(eb, host), receive_period, real_time_fun)));
-    {
-        var replica_index :| replica_index in asp.live_quorum && host == asp.c.config.replica_ids[replica_index];
-        lemma_ReplicaNextPerformsProcessPacketPeriodically(b, asp, replica_index);
-    }
+  forall host | host in destinations
+    ensures sat(asp.synchrony_start, always(eventuallynextwithin(ReceiveAttemptedTemporal(eb, host), receive_period, real_time_fun)))
+  {
+    var replica_index :| replica_index in asp.live_quorum && host == asp.c.config.replica_ids[replica_index];
+    lemma_ReplicaNextPerformsProcessPacketPeriodically(b, asp, replica_index);
+  }
 
-    forall ensures 1 <= receive_period { lemma_mul_inequality_forall(); lemma_mul_auto(); }
-    forall i, j | 0 <= i <= j ensures b[i].environment.time <= b[j].environment.time { lemma_TimeAdvancesBetween(b, asp, i, j); }
-    processing_sync_start, processing_bound := Lemma_EventuallyAllPacketsAlwaysReceivedInTime(asp.synchrony_start, asp.latency_bound, sources, destinations, eb, asp.burst_size, receive_period);
+  forall ensures 1 <= receive_period { lemma_mul_inequality_forall(); lemma_mul_auto(); }
+  forall i, j | 0 <= i <= j ensures b[i].environment.time <= b[j].environment.time { lemma_TimeAdvancesBetween(b, asp, i, j); }
+  processing_sync_start, processing_bound := Lemma_EventuallyAllPacketsAlwaysReceivedInTime(asp.synchrony_start, asp.latency_bound, sources, destinations, eb, asp.burst_size, receive_period);
 }
 
 predicate PacketProcessingSynchronousOneStep(
-    b:Behavior<RslState>,
-    i:int,
-    processing_bound:int,
-    sources:set<NodeIdentity>,
-    destinations:set<NodeIdentity>
-    )
-    requires imaptotal(b);
+  b:Behavior<RslState>,
+  i:int,
+  processing_bound:int,
+  sources:set<NodeIdentity>,
+  destinations:set<NodeIdentity>
+  )
+  requires imaptotal(b)
 {
-    forall p {:trigger PacketSentDuringAction(b[i], p)} ::
-        PacketSentDuringAction(b[i], p) && p.src in sources && p.dst in destinations
-    ==> sat(i, next(eventuallynextwithin(PacketProcessedTemporal(b, p), processing_bound, PaxosTimeMap(b))))
+  forall p {:trigger PacketSentDuringAction(b[i], p)} ::
+      PacketSentDuringAction(b[i], p) && p.src in sources && p.dst in destinations
+      ==> sat(i, next(eventuallynextwithin(PacketProcessedTemporal(b, p), processing_bound, PaxosTimeMap(b))))
 }
 
 function{:opaque} PacketProcessingSynchronousTemporal(
-    b:Behavior<RslState>,
-    processing_bound:int,
-    sources:set<NodeIdentity>,
-    destinations:set<NodeIdentity>
-    ):temporal
-    requires imaptotal(b);
-    ensures  forall i{:trigger sat(i, PacketProcessingSynchronousTemporal(b, processing_bound, sources, destinations))} ::
-        sat(i, PacketProcessingSynchronousTemporal(b, processing_bound, sources, destinations)) <==>
-        PacketProcessingSynchronousOneStep(b, i, processing_bound, sources, destinations);
+  b:Behavior<RslState>,
+  processing_bound:int,
+  sources:set<NodeIdentity>,
+  destinations:set<NodeIdentity>
+  ):temporal
+  requires imaptotal(b)
+  ensures  forall i {:trigger sat(i, PacketProcessingSynchronousTemporal(b, processing_bound, sources, destinations))} ::
+             sat(i, PacketProcessingSynchronousTemporal(b, processing_bound, sources, destinations)) <==>
+             PacketProcessingSynchronousOneStep(b, i, processing_bound, sources, destinations)
 {
-    stepmap(imap i :: PacketProcessingSynchronousOneStep(b, i, processing_bound, sources, destinations))
+  stepmap(imap i :: PacketProcessingSynchronousOneStep(b, i, processing_bound, sources, destinations))
 }
 
 predicate PacketProcessingSynchronous(
-    b:Behavior<RslState>,
-    asp:AssumptionParameters,
-    start_step:int,
-    processing_bound:int
-    )
-    requires LivenessAssumptions(b, asp);
+  b:Behavior<RslState>,
+  asp:AssumptionParameters,
+  start_step:int,
+  processing_bound:int
+  )
+  requires LivenessAssumptions(b, asp)
 {
-    var sources := SetOfReplicaIndicesToSetOfHosts(asp.live_quorum, asp.c.config.replica_ids) + {asp.persistent_request.client};
-    var destinations := SetOfReplicaIndicesToSetOfHosts(asp.live_quorum, asp.c.config.replica_ids);
-       asp.synchrony_start <= start_step
-    && processing_bound >= 0
-    && sat(start_step, always(PacketProcessingSynchronousTemporal(b, processing_bound, sources, destinations)))
+  var sources := SetOfReplicaIndicesToSetOfHosts(asp.live_quorum, asp.c.config.replica_ids) + {asp.persistent_request.client};
+  var destinations := SetOfReplicaIndicesToSetOfHosts(asp.live_quorum, asp.c.config.replica_ids);
+  && asp.synchrony_start <= start_step
+  && processing_bound >= 0
+  && sat(start_step, always(PacketProcessingSynchronousTemporal(b, processing_bound, sources, destinations)))
 }
 
 
 lemma lemma_EventuallyPacketProcessingSynchronous(
-    b:Behavior<RslState>,
-    asp:AssumptionParameters
-    ) returns
-    (processing_sync_start:int,
-     processing_bound:int)
-    requires LivenessAssumptions(b, asp);
-    ensures  PacketProcessingSynchronous(b, asp, processing_sync_start, processing_bound);
+  b:Behavior<RslState>,
+  asp:AssumptionParameters
+  ) returns (
+  processing_sync_start:int,
+  processing_bound:int
+  )
+  requires LivenessAssumptions(b, asp)
+  ensures  PacketProcessingSynchronous(b, asp, processing_sync_start, processing_bound)
 {
-    TemporalAssist();
+  TemporalAssist();
 
-    var eb := RestrictBehaviorToEnvironment(b);
-    var f := PaxosTimeMap(b);
-    var sources := SetOfReplicaIndicesToSetOfHosts(asp.live_quorum, asp.c.config.replica_ids) + {asp.persistent_request.client};
-    var destinations := SetOfReplicaIndicesToSetOfHosts(asp.live_quorum, asp.c.config.replica_ids);
-    var receive_period := TimeToPerformGenericAction(asp);
+  var eb := RestrictBehaviorToEnvironment(b);
+  var f := PaxosTimeMap(b);
+  var sources := SetOfReplicaIndicesToSetOfHosts(asp.live_quorum, asp.c.config.replica_ids) + {asp.persistent_request.client};
+  var destinations := SetOfReplicaIndicesToSetOfHosts(asp.live_quorum, asp.c.config.replica_ids);
+  var receive_period := TimeToPerformGenericAction(asp);
 
-    processing_sync_start, processing_bound := lemma_AllPacketsReceivedInTime(b, asp);
+  processing_sync_start, processing_bound := lemma_AllPacketsReceivedInTime(b, asp);
 
-    forall i | processing_sync_start <= i
-        ensures sat(i, PacketProcessingSynchronousTemporal(b, processing_bound, sources, destinations));
+  forall i | processing_sync_start <= i
+    ensures sat(i, PacketProcessingSynchronousTemporal(b, processing_bound, sources, destinations))
+  {
+    forall p{:trigger PacketSentDuringAction(b[i], p)} | PacketSentDuringAction(b[i], p) && p.src in sources && p.dst in destinations
+      ensures sat(i+1, eventuallynextwithin(PacketProcessedTemporal(b, p), processing_bound, f))
     {
-        forall p{:trigger PacketSentDuringAction(b[i], p)} | PacketSentDuringAction(b[i], p) && p.src in sources && p.dst in destinations
-            ensures sat(i+1, eventuallynextwithin(PacketProcessedTemporal(b, p), processing_bound, f));
-        {
-            TemporalDeduceFromAlways(processing_sync_start, i, AllPacketsReceivedWithinTemporal(eb, processing_bound, sources, destinations));
-            assert PacketSentBetweenHosts(eb[i], p, sources, destinations); // TRIGGER
-            assert sat(i+1, eventuallynextwithin(PacketReceivedTemporal(eb, p), processing_bound, f));
-            var j := TemporalDeduceFromEventual(i+1, nextbefore(PacketReceivedTemporal(eb, p), f[i+1] + processing_bound, f));
-            assert sat(j, PacketReceivedTemporal(eb, p));
-            lemma_PacketReceiveCausesPacketProcessing(b, asp, p, j);
-            assert sat(j, imply(PacketReceivedTemporal(eb, p), PacketProcessedTemporal(b, p)));
-            assert sat(j, PacketProcessedTemporal(b, p));
-            TemporalEventually(i+1, j, nextbefore(PacketProcessedTemporal(b, p), f[i+1] + processing_bound, f));
-        }
+      TemporalDeduceFromAlways(processing_sync_start, i, AllPacketsReceivedWithinTemporal(eb, processing_bound, sources, destinations));
+      assert PacketSentBetweenHosts(eb[i], p, sources, destinations); // TRIGGER
+      assert sat(i, AllPacketsReceivedWithinTemporal(eb, processing_bound, sources, destinations));
+      assert AllPacketsReceivedWithin(eb, i, processing_bound, sources, destinations);
+      assert sat(i, next(eventuallynextwithin(PacketReceivedTemporal(eb, p), processing_bound, f)));
+      var j := TemporalDeduceFromEventual(i+1, nextbefore(PacketReceivedTemporal(eb, p), f[i+1] + processing_bound, f));
+      assert sat(j, PacketReceivedTemporal(eb, p));
+      lemma_PacketReceiveCausesPacketProcessing(b, asp, p, j);
+      assert sat(j, imply(PacketReceivedTemporal(eb, p), PacketProcessedTemporal(b, p)));
+      assert sat(j, PacketProcessedTemporal(b, p));
+      TemporalEventually(i+1, j, nextbefore(PacketProcessedTemporal(b, p), f[i+1] + processing_bound, f));
     }
-    TemporalAlways(processing_sync_start, PacketProcessingSynchronousTemporal(b, processing_bound, sources, destinations));
-    lemma_mul_nonnegative(asp.burst_size, receive_period);
+  }
+  TemporalAlways(processing_sync_start, PacketProcessingSynchronousTemporal(b, processing_bound, sources, destinations));
+  lemma_mul_nonnegative(asp.burst_size, receive_period);
 }
 
 lemma lemma_IfPacketProcessingSynchronousThenAlways(
-    b:Behavior<RslState>,
-    asp:AssumptionParameters,
-    start_step:int,
-    later_step:int,
-    processing_bound:int
-    )
-    requires LivenessAssumptions(b, asp);
-    requires PacketProcessingSynchronous(b, asp, start_step, processing_bound);
-    requires start_step <= later_step;
-    ensures  PacketProcessingSynchronous(b, asp, later_step, processing_bound);
+  b:Behavior<RslState>,
+  asp:AssumptionParameters,
+  start_step:int,
+  later_step:int,
+  processing_bound:int
+  )
+  requires LivenessAssumptions(b, asp)
+  requires PacketProcessingSynchronous(b, asp, start_step, processing_bound)
+  requires start_step <= later_step
+  ensures  PacketProcessingSynchronous(b, asp, later_step, processing_bound)
 {
-    var sources := SetOfReplicaIndicesToSetOfHosts(asp.live_quorum, asp.c.config.replica_ids) + {asp.persistent_request.client};
-    var destinations := SetOfReplicaIndicesToSetOfHosts(asp.live_quorum, asp.c.config.replica_ids);
-    Lemma_AlwaysImpliesLaterAlways(start_step, later_step, PacketProcessingSynchronousTemporal(b, processing_bound, sources, destinations));
+  var sources := SetOfReplicaIndicesToSetOfHosts(asp.live_quorum, asp.c.config.replica_ids) + {asp.persistent_request.client};
+  var destinations := SetOfReplicaIndicesToSetOfHosts(asp.live_quorum, asp.c.config.replica_ids);
+  Lemma_AlwaysImpliesLaterAlways(start_step, later_step, PacketProcessingSynchronousTemporal(b, processing_bound, sources, destinations));
 }
 
 lemma lemma_SchedulerActionThatReceivesReceivesFirst(
-    s:LScheduler,
-    s':LScheduler,
-    p:RslPacket,
-    ios:seq<RslIo>
-    )
-    requires LIoOpReceive(p) in ios;
-    requires LSchedulerNext(s, s', ios);
-    ensures  LIoOpReceive(p) == ios[0];
+  s:LScheduler,
+  s':LScheduler,
+  p:RslPacket,
+  ios:seq<RslIo>
+  )
+  requires LIoOpReceive(p) in ios
+  requires LSchedulerNext(s, s', ios)
+  ensures  LIoOpReceive(p) == ios[0]
 {
-    if LReplicaNextProcessPacket(s.replica, s'.replica, ios)
+  if LReplicaNextProcessPacket(s.replica, s'.replica, ios)
+  {
+    assert ios[0].LIoOpReceive?;
+    if ios[0].r.msg.RslMessage_Heartbeat?
     {
-        assert ios[0].LIoOpReceive?;
-        if ios[0].r.msg.RslMessage_Heartbeat?
-        {
-            assert ios[1].LIoOpReadClock?;
-            assert forall i :: 1 < i < |ios| ==> ios[i].LIoOpSend?;
-            assert LIoOpReceive(p) == ios[0];
-        }
-        else
-        {
-            assert LReplicaNextProcessPacketWithoutReadingClock(s.replica, s'.replica, ios);
-            assert ios[0].LIoOpReceive?;
-            assert forall i :: 0 < i < |ios| ==> ios[i].LIoOpSend?;
-            assert LIoOpReceive(p) == ios[0];
-        }
-    }
-}
-
-lemma lemma_PacketSentToIndexProcessedByIt(
-    b:Behavior<RslState>,
-    asp:AssumptionParameters,
-    processing_sync_start:int,
-    processing_bound:int,
-    send_step:int,
-    idx:int,
-    p:RslPacket
-    )
-    returns(
-    processing_step:int,
-    ios:seq<RslIo>
-    )
-    requires LivenessAssumptions(b, asp);
-    requires idx in asp.live_quorum;
-    requires PacketSentDuringAction(b[send_step], p);
-    requires p.src in SetOfReplicaIndicesToSetOfHosts(asp.live_quorum, asp.c.config.replica_ids) + { asp.persistent_request.client };
-    requires p.dst == asp.c.config.replica_ids[idx];
-    requires PacketProcessingSynchronous(b, asp, processing_sync_start, processing_bound);
-    requires processing_sync_start <= send_step;
-    ensures  send_step+1 <= processing_step;
-    ensures  PacketProcessedViaIos(b[processing_step], b[processing_step+1], p, idx, ios);
-    ensures  b[processing_step+1].environment.time <= b[send_step+1].environment.time + processing_bound;
-{
-    TemporalAssist();
-
-    var timefun := PaxosTimeMap(b);
-
-    assert TLe(processing_sync_start, send_step);
-    processing_step :|    TLe(send_step+1, processing_step)
-                       && sat(processing_step, PacketProcessedTemporal(b, p))
-                       && timefun[processing_step+1] <= timefun[send_step+1] + processing_bound;
-
-    lemma_ConstantsAllConsistent(b, asp.c, processing_step);
-    lemma_ConstantsAllConsistent(b, asp.c, processing_step+1);
-    lemma_AssumptionsMakeValidTransition(b, asp.c, processing_step);
-                       
-    assert b[processing_step].environment.nextStep.LEnvStepHostIos?;
-    ios := b[processing_step].environment.nextStep.ios;
-    var actor := b[processing_step].environment.nextStep.actor;
-    assert p.dst == actor;
-    assert RslNext(b[processing_step], b[processing_step+1]);
-    if exists idx', ios' {:trigger RslNextOneReplica(b[processing_step], b[processing_step+1], idx', ios')} ::
-                     RslNextOneReplica(b[processing_step], b[processing_step+1], idx', ios')
-    {
-        var idx', ios' :| RslNextOneReplica(b[processing_step], b[processing_step+1], idx', ios');
-        assert ReplicasDistinct(asp.c.config.replica_ids, idx, idx');
-        assert idx' == idx && ios' == ios;
-        assert LSchedulerNext(b[processing_step].replicas[idx], b[processing_step+1].replicas[idx], ios);
-        assert LIoOpReceive(p) in ios;
-        lemma_SchedulerActionThatReceivesReceivesFirst(b[processing_step].replicas[idx], b[processing_step+1].replicas[idx], p, ios);
-        assert PacketProcessedViaIos(b[processing_step], b[processing_step+1], p, idx, ios);
-    }
-    else if exists eid, ios' {:trigger RslNextOneExternal(b[processing_step], b[processing_step+1], eid, ios')} ::
-                         RslNextOneExternal(b[processing_step], b[processing_step+1], eid, ios')
-    {
-        var eid, ios' :| RslNextOneExternal(b[processing_step], b[processing_step+1], eid, ios');
-        assert false;
+      assert ios[1].LIoOpReadClock?;
+      assert forall i :: 1 < i < |ios| ==> ios[i].LIoOpSend?;
+      assert LIoOpReceive(p) == ios[0];
     }
     else
     {
-        assert false;
+      assert LReplicaNextProcessPacketWithoutReadingClock(s.replica, s'.replica, ios);
+      assert ios[0].LIoOpReceive?;
+      assert forall i :: 0 < i < |ios| ==> ios[i].LIoOpSend?;
+      assert LIoOpReceive(p) == ios[0];
     }
+  }
+}
+
+lemma lemma_PacketSentToIndexProcessedByIt(
+  b:Behavior<RslState>,
+  asp:AssumptionParameters,
+  processing_sync_start:int,
+  processing_bound:int,
+  send_step:int,
+  idx:int,
+  p:RslPacket
+  ) returns (
+  processing_step:int,
+  ios:seq<RslIo>
+  )
+  requires LivenessAssumptions(b, asp)
+  requires idx in asp.live_quorum
+  requires PacketSentDuringAction(b[send_step], p)
+  requires p.src in SetOfReplicaIndicesToSetOfHosts(asp.live_quorum, asp.c.config.replica_ids) + { asp.persistent_request.client }
+  requires p.dst == asp.c.config.replica_ids[idx]
+  requires PacketProcessingSynchronous(b, asp, processing_sync_start, processing_bound)
+  requires processing_sync_start <= send_step
+  ensures  send_step+1 <= processing_step
+  ensures  PacketProcessedViaIos(b[processing_step], b[processing_step+1], p, idx, ios)
+  ensures  b[processing_step+1].environment.time <= b[send_step+1].environment.time + processing_bound
+{
+  TemporalAssist();
+
+  var timefun := PaxosTimeMap(b);
+
+  assert TLe(processing_sync_start, send_step);
+  processing_step :| && TLe(send_step+1, processing_step)
+                     && sat(processing_step, PacketProcessedTemporal(b, p))
+                     && timefun[processing_step+1] <= timefun[send_step+1] + processing_bound;
+
+  lemma_ConstantsAllConsistent(b, asp.c, processing_step);
+  lemma_ConstantsAllConsistent(b, asp.c, processing_step+1);
+  lemma_AssumptionsMakeValidTransition(b, asp.c, processing_step);
+                       
+  assert b[processing_step].environment.nextStep.LEnvStepHostIos?;
+  ios := b[processing_step].environment.nextStep.ios;
+  var actor := b[processing_step].environment.nextStep.actor;
+  assert p.dst == actor;
+  assert RslNext(b[processing_step], b[processing_step+1]);
+  if exists idx', ios' {:trigger RslNextOneReplica(b[processing_step], b[processing_step+1], idx', ios')} ::
+                  RslNextOneReplica(b[processing_step], b[processing_step+1], idx', ios')
+  {
+    var idx', ios' :| RslNextOneReplica(b[processing_step], b[processing_step+1], idx', ios');
+    assert ReplicasDistinct(asp.c.config.replica_ids, idx, idx');
+    assert idx' == idx && ios' == ios;
+    assert LSchedulerNext(b[processing_step].replicas[idx], b[processing_step+1].replicas[idx], ios);
+    assert LIoOpReceive(p) in ios;
+    lemma_SchedulerActionThatReceivesReceivesFirst(b[processing_step].replicas[idx], b[processing_step+1].replicas[idx], p, ios);
+    assert PacketProcessedViaIos(b[processing_step], b[processing_step+1], p, idx, ios);
+  }
+  else if exists eid, ios' {:trigger RslNextOneExternal(b[processing_step], b[processing_step+1], eid, ios')} ::
+                      RslNextOneExternal(b[processing_step], b[processing_step+1], eid, ios')
+  {
+    var eid, ios' :| RslNextOneExternal(b[processing_step], b[processing_step+1], eid, ios');
+    assert false;
+  }
+  else
+  {
+    assert false;
+  }
 }
 
 } 
