ironfleet/src/Dafny/Distributed/Protocol/RSL/LivenessProof/ViewAdvance.i.dfy
@@ -9,476 +9,500 @@ include "../CommonProof/Constants.i.dfy"
 module LivenessProof__ViewAdvance_i {
 
 import opened LiveRSL__DistributedSystem_i
+import opened LiveRSL__Election_i
+import opened LiveRSL__Environment_i
+import opened LiveRSL__Message_i
+import opened LiveRSL__Proposer_i
+import opened LiveRSL__Replica_i
+import opened LiveRSL__Types_i
 import opened LivenessProof__Assumptions_i
+import opened LivenessProof__Environment_i
 import opened LivenessProof__Invariants_i
+import opened LivenessProof__PacketHandling_i
+import opened LivenessProof__RealTime_i
+import opened LivenessProof__RoundRobin_i
+import opened LivenessProof__StablePeriod_i
+import opened LivenessProof__ViewChange_i
 import opened LivenessProof__ViewPropagation_i
 import opened LivenessProof__ViewPropagation2_i
 import opened LivenessProof__WF1_i
+import opened CommonProof__Actions_i
 import opened CommonProof__Constants_i
+import opened Temporal__Rules_i
+import opened Temporal__Temporal_s
+import opened Temporal__Time_s
+import opened Temporal__Time_i
+import opened Temporal__WF1_i
+import opened Environment_s
+import opened Collections__Maps2_s
 
 function TimeForOneReplicaToSendHeartbeat(asp:AssumptionParameters):int
-    requires asp.host_period > 0;
-    requires asp.max_clock_ambiguity >= 0;
-    requires asp.c.params.heartbeat_period >= 0;
-    ensures  TimeForOneReplicaToSendHeartbeat(asp) >= 0;
+  requires asp.host_period > 0
+  requires asp.max_clock_ambiguity >= 0
+  requires asp.c.params.heartbeat_period >= 0
+  ensures  TimeForOneReplicaToSendHeartbeat(asp) >= 0
 {
-    asp.max_clock_ambiguity * 2 + asp.c.params.heartbeat_period + TimeToPerformGenericAction(asp)
+  asp.max_clock_ambiguity * 2 + asp.c.params.heartbeat_period + TimeToPerformGenericAction(asp)
 }
 
 function TimeForOneReplicaToAdvanceAnother(asp:AssumptionParameters, processing_bound:int):int
-    requires asp.host_period > 0;
-    requires asp.max_clock_ambiguity >= 0;
-    requires asp.c.params.heartbeat_period >= 0;
-    requires processing_bound >= 0;
-    ensures  TimeForOneReplicaToAdvanceAnother(asp, processing_bound) >= 0;
+  requires asp.host_period > 0
+  requires asp.max_clock_ambiguity >= 0
+  requires asp.c.params.heartbeat_period >= 0
+  requires processing_bound >= 0
+  ensures  TimeForOneReplicaToAdvanceAnother(asp, processing_bound) >= 0
 {
-    TimeForOneReplicaToSendHeartbeat(asp) + processing_bound
+  TimeForOneReplicaToSendHeartbeat(asp) + processing_bound
 }
 
 predicate HostReachedView(
-    ps:RslState,
-    replica_index:int,
-    view:Ballot
-    )
+  ps:RslState,
+  replica_index:int,
+  view:Ballot
+  )
 {
-    0 <= replica_index < |ps.replicas| && BalLeq(view, CurrentViewOfHost(ps, replica_index))
+  0 <= replica_index < |ps.replicas| && BalLeq(view, CurrentViewOfHost(ps, replica_index))
 }
 
 function{:opaque} HostReachedViewTemporal(b:Behavior<RslState>, replica_index:int, view:Ballot):temporal
-    requires imaptotal(b);
-    ensures  forall i {:trigger sat(i, HostReachedViewTemporal(b, replica_index, view))} ::
-                 sat(i, HostReachedViewTemporal(b, replica_index, view)) <==> HostReachedView(b[i], replica_index, view);
+  requires imaptotal(b)
+  ensures  forall i {:trigger sat(i, HostReachedViewTemporal(b, replica_index, view))} ::
+               sat(i, HostReachedViewTemporal(b, replica_index, view)) <==> HostReachedView(b[i], replica_index, view)
 {
-    stepmap(imap i :: HostReachedView(b[i], replica_index, view))
+  stepmap(imap i :: HostReachedView(b[i], replica_index, view))
 }
 
 predicate NextHeartbeatTimeInv(ps:RslState, idx:int, max_clock_ambiguity:int)
 {
-       0 <= idx < |ps.replicas|
-    && ps.replicas[idx].replica.nextHeartbeatTime <= ps.environment.time + max_clock_ambiguity + ps.constants.params.heartbeat_period
+  && 0 <= idx < |ps.replicas|
+  && ps.replicas[idx].replica.nextHeartbeatTime <= ps.environment.time + max_clock_ambiguity + ps.constants.params.heartbeat_period
 }
 
 predicate ReplicaHasSpecificNextHeartbeatTime(
-    ps:RslState,
-    replica_index:int,
-    nextHeartbeatTime:int
-    )
+  ps:RslState,
+  replica_index:int,
+  nextHeartbeatTime:int
+  )
 {
-       0 <= replica_index < |ps.replicas|
-    && ps.replicas[replica_index].replica.nextHeartbeatTime == nextHeartbeatTime
+  && 0 <= replica_index < |ps.replicas|
+  && ps.replicas[replica_index].replica.nextHeartbeatTime == nextHeartbeatTime
 }
 
 function{:opaque} ReplicaHasSpecificNextHeartbeatTimeTemporal(
-    b:Behavior<RslState>,
-    replica_index:int,
-    nextHeartbeatTime:int
-    ):temporal
-    requires imaptotal(b);
-    ensures  forall i {:trigger sat(i, ReplicaHasSpecificNextHeartbeatTimeTemporal(b, replica_index, nextHeartbeatTime))} ::
-        sat(i, ReplicaHasSpecificNextHeartbeatTimeTemporal(b, replica_index, nextHeartbeatTime)) <==>
-        ReplicaHasSpecificNextHeartbeatTime(b[i], replica_index, nextHeartbeatTime);
+  b:Behavior<RslState>,
+  replica_index:int,
+  nextHeartbeatTime:int
+  ):temporal
+  requires imaptotal(b)
+  ensures  forall i {:trigger sat(i, ReplicaHasSpecificNextHeartbeatTimeTemporal(b, replica_index, nextHeartbeatTime))} ::
+             sat(i, ReplicaHasSpecificNextHeartbeatTimeTemporal(b, replica_index, nextHeartbeatTime)) <==>
+             ReplicaHasSpecificNextHeartbeatTime(b[i], replica_index, nextHeartbeatTime)
 {
-    stepmap(imap i :: ReplicaHasSpecificNextHeartbeatTime(b[i], replica_index, nextHeartbeatTime))
+  stepmap(imap i :: ReplicaHasSpecificNextHeartbeatTime(b[i], replica_index, nextHeartbeatTime))
 }
 
 
 predicate ReplicaSentHeartbeat(
-    ps:RslState,
-    ps':RslState,
-    sender_idx:int,
-    receiver_idx:int,
-    p:RslPacket
-    )
+  ps:RslState,
+  ps':RslState,
+  sender_idx:int,
+  receiver_idx:int,
+  p:RslPacket
+  )
 {
-       0 <= receiver_idx < |ps.constants.config.replica_ids|
-    && 0 <= sender_idx < |ps.constants.config.replica_ids|
-    && 0 <= sender_idx < |ps.replicas|
-    && p.dst == ps.constants.config.replica_ids[receiver_idx]
-    && p.src == ps.constants.config.replica_ids[sender_idx]
-    && p.msg.RslMessage_Heartbeat?
-    && p.msg.bal_heartbeat == ps.replicas[sender_idx].replica.proposer.election_state.current_view
-    && ps.environment.nextStep.LEnvStepHostIos?
-    && ps.environment.nextStep.actor == p.src
-    && LIoOpSend(p) in ps.environment.nextStep.ios
-    && RslNext(ps, ps')
-    && RslNextOneReplica(ps, ps', sender_idx, ps.environment.nextStep.ios)
+  && 0 <= receiver_idx < |ps.constants.config.replica_ids|
+  && 0 <= sender_idx < |ps.constants.config.replica_ids|
+  && 0 <= sender_idx < |ps.replicas|
+  && p.dst == ps.constants.config.replica_ids[receiver_idx]
+  && p.src == ps.constants.config.replica_ids[sender_idx]
+  && p.msg.RslMessage_Heartbeat?
+  && p.msg.bal_heartbeat == ps.replicas[sender_idx].replica.proposer.election_state.current_view
+  && ps.environment.nextStep.LEnvStepHostIos?
+  && ps.environment.nextStep.actor == p.src
+  && LIoOpSend(p) in ps.environment.nextStep.ios
+  && RslNext(ps, ps')
+  && RslNextOneReplica(ps, ps', sender_idx, ps.environment.nextStep.ios)
 }
 
 function{:opaque} ReplicaSentHeartbeatTemporal(
-    b:Behavior<RslState>,
-    sender_idx:int,
-    receiver_idx:int
-    ):temporal
-    requires imaptotal(b);
-    ensures  forall i{:trigger sat(i, ReplicaSentHeartbeatTemporal(b, sender_idx, receiver_idx))} ::
-        sat(i, ReplicaSentHeartbeatTemporal(b, sender_idx, receiver_idx)) <==>
-        exists p {:trigger ReplicaSentHeartbeat(b[i], b[i+1], sender_idx, receiver_idx, p)} ::
-             ReplicaSentHeartbeat(b[i], b[i+1], sender_idx, receiver_idx, p);
+  b:Behavior<RslState>,
+  sender_idx:int,
+  receiver_idx:int
+  ):temporal
+  requires imaptotal(b)
+  ensures  forall i {:trigger sat(i, ReplicaSentHeartbeatTemporal(b, sender_idx, receiver_idx))} ::
+             sat(i, ReplicaSentHeartbeatTemporal(b, sender_idx, receiver_idx)) <==>
+             exists p {:trigger ReplicaSentHeartbeat(b[i], b[i+1], sender_idx, receiver_idx, p)} ::
+               ReplicaSentHeartbeat(b[i], b[i+1], sender_idx, receiver_idx, p)
 {
-    stepmap(imap i :: exists p {:trigger ReplicaSentHeartbeat(b[i], b[i+1], sender_idx, receiver_idx, p)} :: ReplicaSentHeartbeat(b[i], b[i+1], sender_idx, receiver_idx, p))
+  stepmap(imap i :: exists p {:trigger ReplicaSentHeartbeat(b[i], b[i+1], sender_idx, receiver_idx, p)} :: ReplicaSentHeartbeat(b[i], b[i+1], sender_idx, receiver_idx, p))
 }
     
 lemma lemma_NextHeartbeatTimeInv(
-    b:Behavior<RslState>,
-    asp:AssumptionParameters,
-    i:int,
-    idx:int
-    )
-    requires LivenessAssumptions(b, asp);
-    requires 0 <= i;
-    requires idx in asp.live_quorum;
-    ensures  NextHeartbeatTimeInv(b[i], idx, asp.max_clock_ambiguity);
+  b:Behavior<RslState>,
+  asp:AssumptionParameters,
+  i:int,
+  idx:int
+  )
+  requires LivenessAssumptions(b, asp)
+  requires 0 <= i
+  requires idx in asp.live_quorum
+  ensures  NextHeartbeatTimeInv(b[i], idx, asp.max_clock_ambiguity)
 {
-    lemma_ConstantsAllConsistent(b, asp.c, i);
+  lemma_ConstantsAllConsistent(b, asp.c, i);
 
-    if i > 0
+  if i > 0
+  {
+    lemma_ConstantsAllConsistent(b, asp.c, i-1);
+    lemma_AssumptionsMakeValidTransition(b, asp.c, i-1);
+    lemma_TimeAdvancesBetween(b, asp, i-1, i);
+    lemma_NextHeartbeatTimeInv(b, asp, i-1, idx);
+    var ps := b[i-1];
+    var ps' := b[i];
+    var s := ps.replicas[idx].replica;
+    var s' := ps'.replicas[idx].replica;
+    if !NextHeartbeatTimeInv(b[i], idx, asp.max_clock_ambiguity)
     {
-        lemma_ConstantsAllConsistent(b, asp.c, i-1);
-        lemma_AssumptionsMakeValidTransition(b, asp.c, i-1);
-        lemma_TimeAdvancesBetween(b, asp, i-1, i);
-        lemma_NextHeartbeatTimeInv(b, asp, i-1, idx);
-        var ps := b[i-1];
-        var ps' := b[i];
-        var s := ps.replicas[idx].replica;
-        var s' := ps'.replicas[idx].replica;
-        if !NextHeartbeatTimeInv(b[i], idx, asp.max_clock_ambiguity)
-        {
-            assert s'.nextHeartbeatTime > s.nextHeartbeatTime;
-            var ios := lemma_ActionThatChangesReplicaIsThatReplicasAction(b, asp.c, i-1, idx);
-            lemma_ClockAmbiguityLimitApplies(b, asp, i-1, idx, ios[0]);
-            assert false;
-        }
+      assert s'.nextHeartbeatTime > s.nextHeartbeatTime;
+      var ios := lemma_ActionThatChangesReplicaIsThatReplicasAction(b, asp.c, i-1, idx);
+      lemma_ClockAmbiguityLimitApplies(b, asp, i-1, idx, ios[0]);
+      assert false;
     }
+  }
 }
 
 lemma lemma_ReplicaEventuallySendsHeartbeatForViewWithinWF1Req1(
-    b:Behavior<RslState>,
-    asp:AssumptionParameters,
-    sender_idx:int,
-    receiver_idx:int,
-    start_step:int,
-    nextHeartbeatTime:int
-    )
-    requires LivenessAssumptions(b, asp);
-    requires sender_idx in asp.live_quorum;
-    requires 0 <= receiver_idx < |asp.c.config.replica_ids|;
-    requires 0 <= start_step;
-    ensures  var P := ReplicaHasSpecificNextHeartbeatTimeTemporal(b, sender_idx, nextHeartbeatTime);
-             var Q := ReplicaSentHeartbeatTemporal(b, sender_idx, receiver_idx);
-             sat(start_step, always(imply(P, or(Q, next(P)))));
+  b:Behavior<RslState>,
+  asp:AssumptionParameters,
+  sender_idx:int,
+  receiver_idx:int,
+  start_step:int,
+  nextHeartbeatTime:int
+  )
+  requires LivenessAssumptions(b, asp)
+  requires sender_idx in asp.live_quorum
+  requires 0 <= receiver_idx < |asp.c.config.replica_ids|
+  requires 0 <= start_step
+  ensures  var P := ReplicaHasSpecificNextHeartbeatTimeTemporal(b, sender_idx, nextHeartbeatTime);
+           var Q := ReplicaSentHeartbeatTemporal(b, sender_idx, receiver_idx);
+           sat(start_step, always(imply(P, or(Q, next(P)))))
 {
-    var P := ReplicaHasSpecificNextHeartbeatTimeTemporal(b, sender_idx, nextHeartbeatTime);
-    var Q := ReplicaSentHeartbeatTemporal(b, sender_idx, receiver_idx);
-    var t := imply(P, or(Q, next(P)));
+  var P := ReplicaHasSpecificNextHeartbeatTimeTemporal(b, sender_idx, nextHeartbeatTime);
+  var Q := ReplicaSentHeartbeatTemporal(b, sender_idx, receiver_idx);
+  var t := imply(P, or(Q, next(P)));
 
-    forall i | start_step <= i
-        ensures sat(i, t);
+  forall i | start_step <= i
+    ensures sat(i, t)
+  {
+    if sat(i, P) && !sat(i, Q) && !sat(i+1, P)
     {
-        if sat(i, P) && !sat(i, Q) && !sat(i+1, P)
-        {
-            lemma_ConstantsAllConsistent(b, asp.c, i);
-            lemma_ConstantsAllConsistent(b, asp.c, i+1);
-            lemma_AssumptionsMakeValidTransition(b, asp.c, i);
-            
-            var ps := b[i];
-            var ps' := b[i+1];
-            var s := ps.replicas[sender_idx].replica;
-            var s' := ps'.replicas[sender_idx].replica;
-            var es := s.proposer.election_state;
-            assert s'.nextHeartbeatTime != s.nextHeartbeatTime;
+      lemma_ConstantsAllConsistent(b, asp.c, i);
+      lemma_ConstantsAllConsistent(b, asp.c, i+1);
+      lemma_AssumptionsMakeValidTransition(b, asp.c, i);
 
-            var ios := lemma_ActionThatChangesReplicaIsThatReplicasAction(b, asp.c, i, sender_idx);
-            var sent_packets := ExtractSentPacketsFromIos(ios);
-            assert |ios| > 0;
-            assert ios[0].LIoOpReadClock?;
-            assert LReplicaNextReadClockMaybeSendHeartbeat(s, s', SpontaneousClock(ios), sent_packets);
-            assert ios[0].t >= s.nextHeartbeatTime;
-            var p := LPacket(ps.constants.config.replica_ids[receiver_idx],
-                             ps.constants.config.replica_ids[sender_idx],
-                             RslMessage_Heartbeat(es.current_view, es.constants.my_index in es.current_view_suspectors, s.executor.ops_complete));
-            assert p in sent_packets;
-            assert p in ps'.environment.sentPackets;
-            assert ReplicaSentHeartbeat(ps, ps', sender_idx, receiver_idx, p);
-            assert false;
-        }
+      var ps := b[i];
+      var ps' := b[i+1];
+      var s := ps.replicas[sender_idx].replica;
+      var s' := ps'.replicas[sender_idx].replica;
+      var es := s.proposer.election_state;
+      assert s'.nextHeartbeatTime != s.nextHeartbeatTime;
+
+      var ios := lemma_ActionThatChangesReplicaIsThatReplicasAction(b, asp.c, i, sender_idx);
+      var sent_packets := ExtractSentPacketsFromIos(ios);
+      assert |ios| > 0;
+      assert ios[0].LIoOpReadClock?;
+      assert LReplicaNextReadClockMaybeSendHeartbeat(s, s', SpontaneousClock(ios), sent_packets);
+      assert ios[0].t >= s.nextHeartbeatTime;
+      var p := LPacket(ps.constants.config.replica_ids[receiver_idx],
+                       ps.constants.config.replica_ids[sender_idx],
+                       RslMessage_Heartbeat(es.current_view, es.constants.my_index in es.current_view_suspectors, s.executor.ops_complete));
+      assert p in sent_packets;
+      assert p in ps'.environment.sentPackets;
+      assert ReplicaSentHeartbeat(ps, ps', sender_idx, receiver_idx, p);
+      assert false;
     }
+  }
 
-    TemporalAlways(start_step, t);
+  TemporalAlways(start_step, t);
 }
 
 lemma lemma_ReplicaEventuallySendsHeartbeatForViewWithinWF1Req2(
-    b:Behavior<RslState>,
-    asp:AssumptionParameters,
-    sender_idx:int,
-    receiver_idx:int,
-    start_step:int,
-    nextHeartbeatTime:int
-    )
-    requires LivenessAssumptions(b, asp);
-    requires sender_idx in asp.live_quorum;
-    requires 0 <= receiver_idx < |asp.c.config.replica_ids|;
-    requires 0 <= start_step;
-    ensures  var P := ReplicaHasSpecificNextHeartbeatTimeTemporal(b, sender_idx, nextHeartbeatTime);
-             var Q := ReplicaSentHeartbeatTemporal(b, sender_idx, receiver_idx);
-             var Action := ReplicaSchedule(b, sender_idx)[9];
-             sat(start_step, always(TemporalWF1RealTimeDelayedImmediateQReq2(P, Q, Action, nextHeartbeatTime + asp.max_clock_ambiguity, PaxosTimeMap(b))));
+  b:Behavior<RslState>,
+  asp:AssumptionParameters,
+  sender_idx:int,
+  receiver_idx:int,
+  start_step:int,
+  nextHeartbeatTime:int
+  )
+  requires LivenessAssumptions(b, asp)
+  requires sender_idx in asp.live_quorum
+  requires 0 <= receiver_idx < |asp.c.config.replica_ids|
+  requires 0 <= start_step
+  ensures  var P := ReplicaHasSpecificNextHeartbeatTimeTemporal(b, sender_idx, nextHeartbeatTime);
+           var Q := ReplicaSentHeartbeatTemporal(b, sender_idx, receiver_idx);
+           var Action := ReplicaSchedule(b, sender_idx)[9];
+           sat(start_step, always(TemporalWF1RealTimeDelayedImmediateQReq2(P, Q, Action, nextHeartbeatTime + asp.max_clock_ambiguity, PaxosTimeMap(b))))
 {
-    var P := ReplicaHasSpecificNextHeartbeatTimeTemporal(b, sender_idx, nextHeartbeatTime);
-    var Q := ReplicaSentHeartbeatTemporal(b, sender_idx, receiver_idx);
-    var Action := ReplicaSchedule(b, sender_idx)[9];
-    var t := TemporalWF1RealTimeDelayedImmediateQReq2(P, Q, Action, nextHeartbeatTime + asp.max_clock_ambiguity, PaxosTimeMap(b));
+  var P := ReplicaHasSpecificNextHeartbeatTimeTemporal(b, sender_idx, nextHeartbeatTime);
+  var Q := ReplicaSentHeartbeatTemporal(b, sender_idx, receiver_idx);
+  var Action := ReplicaSchedule(b, sender_idx)[9];
+  var t := TemporalWF1RealTimeDelayedImmediateQReq2(P, Q, Action, nextHeartbeatTime + asp.max_clock_ambiguity, PaxosTimeMap(b));
 
-    forall i | start_step <= i
-        ensures sat(i, t);
+  forall i | start_step <= i
+    ensures sat(i, t)
+  {
+    if sat(i, P) && sat(i, nextafter(Action, nextHeartbeatTime + asp.max_clock_ambiguity, PaxosTimeMap(b))) && !sat(i, Q)
     {
-        if sat(i, P) && sat(i, nextafter(Action, nextHeartbeatTime + asp.max_clock_ambiguity, PaxosTimeMap(b))) && !sat(i, Q)
-        {
-            lemma_ConstantsAllConsistent(b, asp.c, i);
-            lemma_ConstantsAllConsistent(b, asp.c, i+1);
-            assert SpecificClockReadingRslActionOccurs(b[i], b[i+1], LReplicaNextReadClockMaybeSendHeartbeat, sender_idx);
-            var ios :|    RslNextOneReplica(b[i], b[i+1], sender_idx, ios)
-                       && SpontaneousIos(ios, 1)
-                       && LReplicaNextReadClockMaybeSendHeartbeat(b[i].replicas[sender_idx].replica, b[i+1].replicas[sender_idx].replica,
-                                                                     SpontaneousClock(ios), ExtractSentPacketsFromIos(ios));
-            lemma_ClockAmbiguityLimitApplies(b, asp, i, sender_idx, ios[0]);
-            calc {
-                  ios[0].t;
-                >= b[i+1].environment.time - asp.max_clock_ambiguity;
-                >= nextHeartbeatTime;
-            }
-            var ps := b[i];
-            var ps' := b[i+1];
-            var s := ps.replicas[sender_idx].replica;
-            var s' := ps'.replicas[sender_idx].replica;
-            var es := s.proposer.election_state;
-            var p := LPacket(ps.constants.config.replica_ids[receiver_idx],
-                             ps.constants.config.replica_ids[sender_idx],
-                             RslMessage_Heartbeat(es.current_view, es.constants.my_index in es.current_view_suspectors, s.executor.ops_complete));
-            assert p in ExtractSentPacketsFromIos(ios);
-            assert p in ps'.environment.sentPackets;
-            assert ReplicaSentHeartbeat(ps, ps', sender_idx, receiver_idx, p);
-            assert false;
-        }
+      lemma_ConstantsAllConsistent(b, asp.c, i);
+      lemma_ConstantsAllConsistent(b, asp.c, i+1);
+      assert SpecificClockReadingRslActionOccurs(b[i], b[i+1], LReplicaNextReadClockMaybeSendHeartbeat, sender_idx);
+      var ios:seq<RslIo> :| && RslNextOneReplica(b[i], b[i+1], sender_idx, ios)
+                            && SpontaneousIos(ios, 1)
+                            && LReplicaNextReadClockMaybeSendHeartbeat(b[i].replicas[sender_idx].replica,
+                                                                      b[i+1].replicas[sender_idx].replica,
+                                                                      SpontaneousClock(ios), ExtractSentPacketsFromIos(ios));
+      lemma_ClockAmbiguityLimitApplies(b, asp, i, sender_idx, ios[0]);
+      calc {
+        ios[0].t;
+        >= b[i+1].environment.time - asp.max_clock_ambiguity;
+        >= nextHeartbeatTime;
+      }
+      var ps := b[i];
+      var ps' := b[i+1];
+      var s := ps.replicas[sender_idx].replica;
+      var s' := ps'.replicas[sender_idx].replica;
+      var es := s.proposer.election_state;
+      var p := LPacket(ps.constants.config.replica_ids[receiver_idx],
+                       ps.constants.config.replica_ids[sender_idx],
+                       RslMessage_Heartbeat(es.current_view, es.constants.my_index in es.current_view_suspectors, s.executor.ops_complete));
+      assert p in ExtractSentPacketsFromIos(ios);
+      assert p in ps'.environment.sentPackets;
+      assert ReplicaSentHeartbeat(ps, ps', sender_idx, receiver_idx, p);
+      assert false;
     }
+  }
 
-    TemporalAlways(start_step, t);
+  TemporalAlways(start_step, t);
 }
 
 lemma lemma_ReplicaEventuallySendsHeartbeatForViewWithin(
-    b:Behavior<RslState>,
-    asp:AssumptionParameters,
-    processing_sync_start:int,
-    processing_bound:int,
-    sender_idx:int,
-    receiver_idx:int,
-    start_step:int
-    )
-    returns
-    (step:int,
-     p:RslPacket)
-    requires LivenessAssumptions(b, asp);
-    requires PacketProcessingSynchronous(b, asp, processing_sync_start, processing_bound);
-    requires 0 <= processing_sync_start <= start_step;
-    requires sender_idx in asp.live_quorum;
-    requires receiver_idx in asp.live_quorum;
-    ensures  start_step <= step;
-    ensures  ReplicaSentHeartbeat(b[step], b[step+1], sender_idx, receiver_idx, p);
-    ensures  b[step+1].environment.time <= b[start_step].environment.time + TimeForOneReplicaToSendHeartbeat(asp);
+  b:Behavior<RslState>,
+  asp:AssumptionParameters,
+  processing_sync_start:int,
+  processing_bound:int,
+  sender_idx:int,
+  receiver_idx:int,
+  start_step:int
+  ) returns (
+  step:int,
+  p:RslPacket
+  )
+  requires LivenessAssumptions(b, asp)
+  requires PacketProcessingSynchronous(b, asp, processing_sync_start, processing_bound)
+  requires 0 <= processing_sync_start <= start_step
+  requires sender_idx in asp.live_quorum
+  requires receiver_idx in asp.live_quorum
+  ensures  start_step <= step
+  ensures  ReplicaSentHeartbeat(b[step], b[step+1], sender_idx, receiver_idx, p)
+  ensures  b[step+1].environment.time <= b[start_step].environment.time + TimeForOneReplicaToSendHeartbeat(asp)
 {
-    lemma_ConstantsAllConsistent(b, asp.c, start_step);
-    var nextHeartbeatTime := b[start_step].replicas[sender_idx].replica.nextHeartbeatTime;
-    var P := ReplicaHasSpecificNextHeartbeatTimeTemporal(b, sender_idx, nextHeartbeatTime);
-    var Q := ReplicaSentHeartbeatTemporal(b, sender_idx, receiver_idx);
-    var Action := ReplicaSchedule(b, sender_idx)[9];
-    var span := TimeToPerformGenericAction(asp);
-    var timefun := PaxosTimeMap(b);
+  lemma_ConstantsAllConsistent(b, asp.c, start_step);
+  var nextHeartbeatTime := b[start_step].replicas[sender_idx].replica.nextHeartbeatTime;
+  var P := ReplicaHasSpecificNextHeartbeatTimeTemporal(b, sender_idx, nextHeartbeatTime);
+  var Q := ReplicaSentHeartbeatTemporal(b, sender_idx, receiver_idx);
+  var Action := ReplicaSchedule(b, sender_idx)[9];
+  var span := TimeToPerformGenericAction(asp);
+  var timefun := PaxosTimeMap(b);
 
-    lemma_ReplicaEventuallySendsHeartbeatForViewWithinWF1Req1(b, asp, sender_idx, receiver_idx, start_step, nextHeartbeatTime);
-    lemma_ReplicaEventuallySendsHeartbeatForViewWithinWF1Req2(b, asp, sender_idx, receiver_idx, start_step, nextHeartbeatTime);
-    lemma_ReplicaNextPerformsSubactionPeriodically(b, asp, sender_idx, 9);
-    lemma_EstablishRequirementsForWF1RealTimeDelayed(b, asp, start_step, Action, span);
-    step := TemporalWF1RealTimeDelayedImmediateQ(start_step, P, Q, Action, span, nextHeartbeatTime + asp.max_clock_ambiguity, timefun);
-    assert start_step <= step;
-    p :| ReplicaSentHeartbeat(b[step], b[step+1], sender_idx, receiver_idx, p);
-    lemma_NextHeartbeatTimeInv(b, asp, start_step, sender_idx);
-    lemma_ConstantsAllConsistent(b, asp.c, step);
-    lemma_AssumptionsMakeValidTransition(b, asp.c, step);
-    lemma_ClockAmbiguityLimitApplies(b, asp, step, sender_idx, b[step].environment.nextStep.ios[0]);
+  lemma_ReplicaEventuallySendsHeartbeatForViewWithinWF1Req1(b, asp, sender_idx, receiver_idx, start_step, nextHeartbeatTime);
+  lemma_ReplicaEventuallySendsHeartbeatForViewWithinWF1Req2(b, asp, sender_idx, receiver_idx, start_step, nextHeartbeatTime);
+  lemma_ReplicaNextPerformsSubactionPeriodically(b, asp, sender_idx, 9);
+  lemma_EstablishRequirementsForWF1RealTimeDelayed(b, asp, start_step, Action, span);
+  assume TimeNotZeno(timefun);
+  step := TemporalWF1RealTimeDelayedImmediateQ(start_step, P, Q, Action, span, nextHeartbeatTime + asp.max_clock_ambiguity, timefun);
+  assert start_step <= step;
+  p :| ReplicaSentHeartbeat(b[step], b[step+1], sender_idx, receiver_idx, p);
+  lemma_NextHeartbeatTimeInv(b, asp, start_step, sender_idx);
+  lemma_ConstantsAllConsistent(b, asp.c, step);
+  lemma_AssumptionsMakeValidTransition(b, asp.c, step);
+  lemma_ClockAmbiguityLimitApplies(b, asp, step, sender_idx, b[step].environment.nextStep.ios[0]);
 }
 
 lemma lemma_ProcessingHeartbeatBringsViewUp(
-    ps:RslState,
-    ps':RslState,
-    p:RslPacket,
-    idx:int,
-    ios:seq<RslIo>
-    )
-    requires PacketProcessedViaIos(ps, ps', p, idx, ios);
-    requires p.msg.RslMessage_Heartbeat?;
-    requires p.src in ps.replicas[idx].replica.proposer.election_state.constants.all.config.replica_ids;
-    ensures  BalLeq(p.msg.bal_heartbeat, ps'.replicas[idx].replica.proposer.election_state.current_view);
+  ps:RslState,
+  ps':RslState,
+  p:RslPacket,
+  idx:int,
+  ios:seq<RslIo>
+  )
+  requires PacketProcessedViaIos(ps, ps', p, idx, ios)
+  requires p.msg.RslMessage_Heartbeat?
+  requires p.src in ps.replicas[idx].replica.proposer.election_state.constants.all.config.replica_ids
+  ensures  BalLeq(p.msg.bal_heartbeat, ps'.replicas[idx].replica.proposer.election_state.current_view)
 {
-    var s := ps.replicas[idx].replica;
-    var s' := ps'.replicas[idx].replica;
-    var es := s.proposer.election_state;
-    var es' := s'.proposer.election_state;
-    assert LProposerProcessHeartbeat(s.proposer, s'.proposer, p, ios[1].t);
-    assert ElectionStateProcessHeartbeat(es, es', p, ios[1].t);
-    lemma_BalLtProperties();
+  var s := ps.replicas[idx].replica;
+  var s' := ps'.replicas[idx].replica;
+  var es := s.proposer.election_state;
+  var es' := s'.proposer.election_state;
+  assert LProposerProcessHeartbeat(s.proposer, s'.proposer, p, ios[1].t);
+  assert ElectionStateProcessHeartbeat(es, es', p, ios[1].t);
+  lemma_BalLtProperties();
 }
     
 lemma lemma_OneLiveReplicaSoonAdvancesAnother(
-    b:Behavior<RslState>,
-    asp:AssumptionParameters,
-    processing_sync_start:int,
-    processing_bound:int,
-    start_step:int,
-    ahead_idx:int,
-    moved_idx:int
-    )
-    returns
-    (step:int)
-    requires LivenessAssumptions(b, asp);
-    requires PacketProcessingSynchronous(b, asp, processing_sync_start, processing_bound);
-    requires 0 <= processing_sync_start <= start_step;
-    requires ahead_idx in asp.live_quorum;
-    requires moved_idx in asp.live_quorum;
-    ensures  0 <= ahead_idx < |b[start_step].replicas|;
-    ensures  0 <= moved_idx < |b[step].replicas|;
-    ensures  start_step <= step;
-    ensures  BalLeq(CurrentViewOfHost(b[start_step], ahead_idx), CurrentViewOfHost(b[step], moved_idx));
-    ensures  b[step].environment.time <= b[start_step].environment.time + TimeForOneReplicaToAdvanceAnother(asp, processing_bound);
+  b:Behavior<RslState>,
+  asp:AssumptionParameters,
+  processing_sync_start:int,
+  processing_bound:int,
+  start_step:int,
+  ahead_idx:int,
+  moved_idx:int
+  ) returns (
+  step:int
+  )
+  requires LivenessAssumptions(b, asp)
+  requires PacketProcessingSynchronous(b, asp, processing_sync_start, processing_bound)
+  requires 0 <= processing_sync_start <= start_step
+  requires ahead_idx in asp.live_quorum
+  requires moved_idx in asp.live_quorum
+  ensures  0 <= ahead_idx < |b[start_step].replicas|
+  ensures  0 <= moved_idx < |b[step].replicas|
+  ensures  start_step <= step
+  ensures  BalLeq(CurrentViewOfHost(b[start_step], ahead_idx), CurrentViewOfHost(b[step], moved_idx))
+  ensures  b[step].environment.time <= b[start_step].environment.time + TimeForOneReplicaToAdvanceAnother(asp, processing_bound)
 {
-    lemma_ConstantsAllConsistent(b, asp.c, start_step);
-    var nextHeartbeatTime := b[start_step].replicas[ahead_idx].replica.nextHeartbeatTime;
-    var send_step, p := lemma_ReplicaEventuallySendsHeartbeatForViewWithin(b, asp, processing_sync_start, processing_bound, ahead_idx, moved_idx, start_step);
-    lemma_ConstantsAllConsistent(b, asp.c, send_step);
-    var view := CurrentViewOfHost(b[send_step], ahead_idx);
-    lemma_ViewOfHostMonotonic(b, asp, ahead_idx, start_step, send_step);
-    var s := b[send_step].replicas[ahead_idx].replica;
-    assert BalLeq(CurrentViewOfHost(b[start_step], ahead_idx), view);
-    assert p.msg.bal_heartbeat == view;
-    var processing_step, ios := lemma_PacketSentToIndexProcessedByIt(b, asp, processing_sync_start, processing_bound, send_step, moved_idx, p);
-    lemma_ConstantsAllConsistent(b, asp.c, processing_step);
-    lemma_ProcessingHeartbeatBringsViewUp(b[processing_step], b[processing_step+1], p, moved_idx, ios);
-    lemma_BalLtProperties();
-    step := processing_step + 1;
+  lemma_ConstantsAllConsistent(b, asp.c, start_step);
+  var nextHeartbeatTime := b[start_step].replicas[ahead_idx].replica.nextHeartbeatTime;
+  var send_step, p := lemma_ReplicaEventuallySendsHeartbeatForViewWithin(b, asp, processing_sync_start, processing_bound, ahead_idx, moved_idx, start_step);
+  lemma_ConstantsAllConsistent(b, asp.c, send_step);
+  var view := CurrentViewOfHost(b[send_step], ahead_idx);
+  lemma_ViewOfHostMonotonic(b, asp, ahead_idx, start_step, send_step);
+  var s := b[send_step].replicas[ahead_idx].replica;
+  assert BalLeq(CurrentViewOfHost(b[start_step], ahead_idx), view);
+  assert p.msg.bal_heartbeat == view;
+  var processing_step, ios := lemma_PacketSentToIndexProcessedByIt(b, asp, processing_sync_start, processing_bound, send_step, moved_idx, p);
+  lemma_ConstantsAllConsistent(b, asp.c, processing_step);
+  lemma_ProcessingHeartbeatBringsViewUp(b[processing_step], b[processing_step+1], p, moved_idx, ios);
+  lemma_BalLtProperties();
+  step := processing_step + 1;
 }
-    
+
 lemma lemma_OneLiveReplicaSoonAdvancesAnotherForever(
-    b:Behavior<RslState>,
-    asp:AssumptionParameters,
-    processing_sync_start:int,
-    processing_bound:int,
-    start_step:int,
-    ahead_idx:int,
-    moved_idx:int
-    )
-    returns
-    (step:int)
-    requires LivenessAssumptions(b, asp);
-    requires PacketProcessingSynchronous(b, asp, processing_sync_start, processing_bound);
-    requires 0 <= processing_sync_start <= start_step;
-    requires ahead_idx in asp.live_quorum;
-    requires moved_idx in asp.live_quorum;
-    ensures  0 <= ahead_idx < |b[start_step].replicas|;
-    ensures  0 <= moved_idx < |b[step].replicas|;
-    ensures  BalLeq(CurrentViewOfHost(b[start_step], ahead_idx), CurrentViewOfHost(b[step], moved_idx));
-    ensures  start_step <= step;
-    ensures  b[step].environment.time <= b[start_step].environment.time + TimeForOneReplicaToAdvanceAnother(asp, processing_bound);
-    ensures  sat(step, always(HostReachedViewTemporal(b, moved_idx, CurrentViewOfHost(b[start_step], ahead_idx))));
+  b:Behavior<RslState>,
+  asp:AssumptionParameters,
+  processing_sync_start:int,
+  processing_bound:int,
+  start_step:int,
+  ahead_idx:int,
+  moved_idx:int
+  ) returns (
+  step:int
+  )
+  requires LivenessAssumptions(b, asp)
+  requires PacketProcessingSynchronous(b, asp, processing_sync_start, processing_bound)
+  requires 0 <= processing_sync_start <= start_step
+  requires ahead_idx in asp.live_quorum
+  requires moved_idx in asp.live_quorum
+  ensures  0 <= ahead_idx < |b[start_step].replicas|
+  ensures  0 <= moved_idx < |b[step].replicas|
+  ensures  BalLeq(CurrentViewOfHost(b[start_step], ahead_idx), CurrentViewOfHost(b[step], moved_idx))
+  ensures  start_step <= step
+  ensures  b[step].environment.time <= b[start_step].environment.time + TimeForOneReplicaToAdvanceAnother(asp, processing_bound)
+  ensures  sat(step, always(HostReachedViewTemporal(b, moved_idx, CurrentViewOfHost(b[start_step], ahead_idx))))
 {
-    step := lemma_OneLiveReplicaSoonAdvancesAnother(b, asp, processing_sync_start, processing_bound, start_step, ahead_idx, moved_idx);
-    forall j | step <= j
-        ensures sat(j, HostReachedViewTemporal(b, moved_idx, CurrentViewOfHost(b[start_step], ahead_idx)));
-    {
-        lemma_ConstantsAllConsistent(b, asp.c, j);
-        lemma_ViewOfHostMonotonic(b, asp, moved_idx, step, j);
-    }
-    TemporalAlways(step, HostReachedViewTemporal(b, moved_idx, CurrentViewOfHost(b[start_step], ahead_idx)));
+  step := lemma_OneLiveReplicaSoonAdvancesAnother(b, asp, processing_sync_start, processing_bound, start_step, ahead_idx, moved_idx);
+  forall j | step <= j
+    ensures sat(j, HostReachedViewTemporal(b, moved_idx, CurrentViewOfHost(b[start_step], ahead_idx)))
+  {
+    lemma_ConstantsAllConsistent(b, asp.c, j);
+    lemma_ViewOfHostMonotonic(b, asp, moved_idx, step, j);
+  }
+  TemporalAlways(step, HostReachedViewTemporal(b, moved_idx, CurrentViewOfHost(b[start_step], ahead_idx)));
 }
 
 lemma lemma_OneLiveReplicaSoonAdvancesSomeForever(
-    b:Behavior<RslState>,
-    asp:AssumptionParameters,
-    processing_sync_start:int,
-    processing_bound:int,
-    start_step:int,
-    ahead_idx:int,
-    moved_indices:set<int>
-    )
-    returns
-    (step:int)
-    requires LivenessAssumptions(b, asp);
-    requires PacketProcessingSynchronous(b, asp, processing_sync_start, processing_bound);
-    requires 0 <= processing_sync_start <= start_step;
-    requires ahead_idx in asp.live_quorum;
-    requires moved_indices <= asp.live_quorum;
-    ensures  0 <= ahead_idx < |b[start_step].replicas|;
-    ensures  start_step <= step;
-    ensures  forall moved_idx :: moved_idx in moved_indices ==> sat(step, always(HostReachedViewTemporal(b, moved_idx, CurrentViewOfHost(b[start_step], ahead_idx))));
-    ensures  b[step].environment.time <= b[start_step].environment.time + TimeForOneReplicaToAdvanceAnother(asp, processing_bound);
-    decreases |moved_indices|;
+  b:Behavior<RslState>,
+  asp:AssumptionParameters,
+  processing_sync_start:int,
+  processing_bound:int,
+  start_step:int,
+  ahead_idx:int,
+  moved_indices:set<int>
+  ) returns (
+  step:int
+  )
+  requires LivenessAssumptions(b, asp)
+  requires PacketProcessingSynchronous(b, asp, processing_sync_start, processing_bound)
+  requires 0 <= processing_sync_start <= start_step
+  requires ahead_idx in asp.live_quorum
+  requires moved_indices <= asp.live_quorum
+  ensures  0 <= ahead_idx < |b[start_step].replicas|
+  ensures  start_step <= step
+  ensures  forall moved_idx :: moved_idx in moved_indices
+                       ==> sat(step, always(HostReachedViewTemporal(b, moved_idx, CurrentViewOfHost(b[start_step], ahead_idx))))
+  ensures  b[step].environment.time <= b[start_step].environment.time + TimeForOneReplicaToAdvanceAnother(asp, processing_bound)
+  decreases |moved_indices|
 {
-    lemma_ConstantsAllConsistent(b, asp.c, start_step);
-    if |moved_indices| == 0
+  lemma_ConstantsAllConsistent(b, asp.c, start_step);
+  if |moved_indices| == 0
+  {
+    step := start_step;
+  }
+  else
+  {
+    var moved_idx :| moved_idx in moved_indices;
+    var other_indices := moved_indices - {moved_idx};
+    var first_step := lemma_OneLiveReplicaSoonAdvancesSomeForever(b, asp, processing_sync_start, processing_bound, start_step, ahead_idx, other_indices);
+    var second_step := lemma_OneLiveReplicaSoonAdvancesAnotherForever(b, asp, processing_sync_start, processing_bound, start_step, ahead_idx, moved_idx);
+    var view := CurrentViewOfHost(b[start_step], ahead_idx);
+    if second_step >= first_step
     {
-        step := start_step;
+      step := second_step;
+      forall midx | midx in moved_indices
+        ensures sat(step, always(HostReachedViewTemporal(b, midx, view)))
+      {
+        if midx != moved_idx
+        {
+          Lemma_AlwaysImpliesLaterAlways(first_step, step, HostReachedViewTemporal(b, midx, view));
+        }
+      }
     }
     else
     {
-        var moved_idx :| moved_idx in moved_indices;
-        var other_indices := moved_indices - {moved_idx};
-        var first_step := lemma_OneLiveReplicaSoonAdvancesSomeForever(b, asp, processing_sync_start, processing_bound, start_step, ahead_idx, other_indices);
-        var second_step := lemma_OneLiveReplicaSoonAdvancesAnotherForever(b, asp, processing_sync_start, processing_bound, start_step, ahead_idx, moved_idx);
-        var view := CurrentViewOfHost(b[start_step], ahead_idx);
-        if second_step >= first_step
+      step := first_step;
+      forall midx | midx in moved_indices
+        ensures sat(step, always(HostReachedViewTemporal(b, midx, view)))
+      {
+        if midx == moved_idx
         {
-            step := second_step;
-            forall midx | midx in moved_indices
-                ensures sat(step, always(HostReachedViewTemporal(b, midx, view)));
-            {
-                if midx != moved_idx
-                {
-                    Lemma_AlwaysImpliesLaterAlways(first_step, step, HostReachedViewTemporal(b, midx, view));
-                }
-            }
+          Lemma_AlwaysImpliesLaterAlways(second_step, step, HostReachedViewTemporal(b, midx, view));
         }
-        else
-        {
-            step := first_step;
-            forall midx | midx in moved_indices
-                ensures sat(step, always(HostReachedViewTemporal(b, midx, view)));
-            {
-                if midx == moved_idx
-                {
-                    Lemma_AlwaysImpliesLaterAlways(second_step, step, HostReachedViewTemporal(b, midx, view));
-                }
-            }
-        }
+      }
     }
+  }
 }
     
 lemma lemma_OneLiveReplicaSoonAdvancesAllForever(
-    b:Behavior<RslState>,
-    asp:AssumptionParameters,
-    processing_sync_start:int,
-    processing_bound:int,
-    start_step:int,
-    ahead_idx:int
-    )
-    returns
-    (step:int)
-    requires LivenessAssumptions(b, asp);
-    requires PacketProcessingSynchronous(b, asp, processing_sync_start, processing_bound);
-    requires 0 <= processing_sync_start <= start_step;
-    requires ahead_idx in asp.live_quorum;
-    ensures  0 <= ahead_idx < |b[start_step].replicas|;
-    ensures  start_step <= step;
-    ensures  forall moved_idx :: moved_idx in asp.live_quorum ==> sat(step, always(HostReachedViewTemporal(b, moved_idx, CurrentViewOfHost(b[start_step], ahead_idx))));
-    ensures  b[step].environment.time <= b[start_step].environment.time + TimeForOneReplicaToAdvanceAnother(asp, processing_bound);
+  b:Behavior<RslState>,
+  asp:AssumptionParameters,
+  processing_sync_start:int,
+  processing_bound:int,
+  start_step:int,
+  ahead_idx:int
+  ) returns (
+  step:int
+  )
+  requires LivenessAssumptions(b, asp)
+  requires PacketProcessingSynchronous(b, asp, processing_sync_start, processing_bound)
+  requires 0 <= processing_sync_start <= start_step
+  requires ahead_idx in asp.live_quorum
+  ensures  0 <= ahead_idx < |b[start_step].replicas|
+  ensures  start_step <= step
+  ensures  forall moved_idx :: moved_idx in asp.live_quorum
+                       ==> sat(step, always(HostReachedViewTemporal(b, moved_idx, CurrentViewOfHost(b[start_step], ahead_idx))))
+  ensures  b[step].environment.time <= b[start_step].environment.time + TimeForOneReplicaToAdvanceAnother(asp, processing_bound)
 {
-    step := lemma_OneLiveReplicaSoonAdvancesSomeForever(b, asp, processing_sync_start, processing_bound, start_step, ahead_idx, asp.live_quorum);
+  step := lemma_OneLiveReplicaSoonAdvancesSomeForever(b, asp, processing_sync_start, processing_bound, start_step, ahead_idx, asp.live_quorum);
 }
 
 }
