ironfleet/src/Dafny/Distributed/Protocol/RSL/LivenessProof/RequestQueue.i.dfy
@@ -5,62 +5,77 @@ include "../CommonProof/Actions.i.dfy"
 
 module LivenessProof__RequestQueue_i {
 
+import opened LiveRSL__DistributedSystem_i
+import opened LiveRSL__Environment_i
+import opened LiveRSL__Types_i
 import opened LivenessProof__Assumptions_i
+import opened LivenessProof__Environment_i
 import opened LivenessProof__Invariants_i
 import opened CommonProof__Actions_i
+import opened CommonProof__Constants_i
 import opened LivenessProof__StablePeriod_i
+import opened Temporal__Temporal_s
+import opened Temporal__Rules_i
+import opened Environment_s
+import opened Collections__Maps2_s
 
 lemma lemma_RequestInFirstNOfRequestQueueDuringPhase1(
-    b:Behavior<RslState>,
-    asp:AssumptionParameters,
-    i:int,
-    start_step:int,
-    view:Ballot,
-    ahead_idx:int,
-    req:Request,
-    n:int
-    )
-    requires LivenessAssumptions(b, asp);
-    requires sat(start_step, StablePeriodStartedTemporal(b, asp.live_quorum, view, ahead_idx));
-    requires sat(start_step, always(RequestInFirstNTemporal(b, view.proposer_id, req, n)));
-    requires 0 <= start_step <= i;
-    requires 0 <= view.proposer_id < |b[i].replicas|;
-    requires b[i].replicas[view.proposer_id].replica.proposer.max_ballot_i_sent_1a == view;
-    requires b[i].replicas[view.proposer_id].replica.proposer.current_state == 1;
-    ensures  RequestInFirstNOfRequestQueue(b[i], view.proposer_id, req, n);
+  b:Behavior<RslState>,
+  asp:AssumptionParameters,
+  i:int,
+  start_step:int,
+  view:Ballot,
+  ahead_idx:int,
+  req:Request,
+  n:int
+  )
+  requires LivenessAssumptions(b, asp)
+  requires sat(start_step, StablePeriodStartedTemporal(b, asp.live_quorum, view, ahead_idx))
+  requires sat(start_step, always(RequestInFirstNTemporal(b, view.proposer_id, req, n)))
+  requires 0 <= start_step <= i
+  requires 0 <= view.proposer_id < |b[i].replicas|
+  requires b[i].replicas[view.proposer_id].replica.proposer.max_ballot_i_sent_1a == view
+  requires b[i].replicas[view.proposer_id].replica.proposer.current_state == 1
+  ensures  RequestInFirstNOfRequestQueue(b[i], view.proposer_id, req, n)
 {
-    if i == start_step
+  if i == start_step
+  {
+    assert false;
+  }
+  else
+  {
+    lemma_ConstantsAllConsistent(b, asp.c, i-1);
+    lemma_ConstantsAllConsistent(b, asp.c, i);
+    lemma_AssumptionsMakeValidTransition(b, asp.c, i-1);
+
+    var idx := view.proposer_id;
+    var s := b[i-1].replicas[idx].replica.proposer;
+    var s' := b[i].replicas[idx].replica.proposer;
+
+    if s.max_ballot_i_sent_1a == view && s.current_state == 1
     {
-        assert false;
+      lemma_RequestInFirstNOfRequestQueueDuringPhase1(b, asp, i-1, start_step, view, ahead_idx, req, n);
+      if s'.request_queue == s.request_queue
+      {
+        assert RequestInFirstNOfRequestQueue(b[i], idx, req, n);
+      }
+      else
+      {
+        var ios := lemma_ActionThatChangesReplicaIsThatReplicasAction(b, asp.c, i-1, idx);
+        var action_index := b[i-1].replicas[idx].nextActionIndex;
+        assert action_index == 0 && ios[0].LIoOpReceive? && ios[0].r.msg.RslMessage_Request?;
+        assert s.request_queue <= s'.request_queue;
+      }
     }
     else
     {
-        lemma_ConstantsAllConsistent(b, asp.c, i-1);
-        lemma_ConstantsAllConsistent(b, asp.c, i);
-        lemma_AssumptionsMakeValidTransition(b, asp.c, i-1);
-
-        var idx := view.proposer_id;
-        var s := b[i-1].replicas[idx].replica.proposer;
-        var s' := b[i].replicas[idx].replica.proposer;
-
-        if s.max_ballot_i_sent_1a == view && s.current_state == 1
-        {
-            lemma_RequestInFirstNOfRequestQueueDuringPhase1(b, asp, i-1, start_step, view, ahead_idx, req, n);
-            if s'.request_queue == s.request_queue
-            {
-                assert RequestInFirstNOfRequestQueue(b[i], idx, req, n);
-            }
-            else
-            {
-                var ios := lemma_ActionThatChangesReplicaIsThatReplicasAction(b, asp.c, i-1, idx);
-            }
-        }
-        else
-        {
-            var ios := lemma_ActionThatChangesReplicaIsThatReplicasAction(b, asp.c, i-1, idx);
-            TemporalDeduceFromAlways(start_step, i-1, RequestInFirstNTemporal(b, idx, req, n));
-        }
+      var ios := lemma_ActionThatChangesReplicaIsThatReplicasAction(b, asp.c, i-1, idx);
+      TemporalDeduceFromAlways(start_step, i-1, RequestInFirstNTemporal(b, idx, req, n));
+      var action_index := b[i-1].replicas[idx].nextActionIndex;
+      assert action_index == 1;
+      assert s.election_state.requests_received_prev_epochs <= s'.request_queue;
     }
+  }
 }
 
 }
