ironfleet/src/Dafny/Distributed/Protocol/RSL/LivenessProof/WF1.i.dfy
@@ -4,45 +4,54 @@ include "../../../Common/Logic/Temporal/WF1.i.dfy"
 include "../CommonProof/Actions.i.dfy"
 
 module LivenessProof__WF1_i {
+import opened LiveRSL__DistributedSystem_i
+import opened LivenessProof__Assumptions_i
 import opened LivenessProof__Invariants_i
 import opened LivenessProof__RealTime_i
 import opened CommonProof__Actions_i
+import opened Temporal__Rules_i
+import opened Temporal__Temporal_s
+import opened Temporal__Time_s
+import opened Temporal__Time_i
 import opened Temporal__WF1_i
+import opened Collections__Maps2_i
 
 lemma lemma_EstablishRequirementsForWF1RealTimeDelayed(
-    b:Behavior<RslState>,
-    asp:AssumptionParameters,
-    i:int,
-    action:temporal,
-    span:int
-    )
-    requires LivenessAssumptions(b, asp);
-    requires asp.synchrony_start <= i;
-    requires sat(asp.synchrony_start, always(eventuallynextwithin(action, span, PaxosTimeMap(b))));
-    ensures  sat(i, always(eventuallynextwithin(action, span, PaxosTimeMap(b))));
-    ensures  monotonic_from(0, PaxosTimeMap(b));
-    ensures  forall t :: sat(0, eventual(after(t, PaxosTimeMap(b))));
+  b:Behavior<RslState>,
+  asp:AssumptionParameters,
+  i:int,
+  action:temporal,
+  span:int
+  )
+  requires LivenessAssumptions(b, asp)
+  requires asp.synchrony_start <= i
+  requires sat(asp.synchrony_start, always(eventuallynextwithin(action, span, PaxosTimeMap(b))))
+  ensures  sat(i, always(eventuallynextwithin(action, span, PaxosTimeMap(b))))
+  ensures  monotonic_from(0, PaxosTimeMap(b))
+  ensures  TimeNotZeno(PaxosTimeMap(b))
 {
-    lemma_TimeMonotonicFromInvariantHolds(b, asp, 0);
-    lemma_AfterForm(b, asp);
-    Lemma_AlwaysImpliesLaterAlways(asp.synchrony_start, i, eventuallynextwithin(action, span, PaxosTimeMap(b)));
+  lemma_TimeMonotonicFromInvariantHolds(b, asp, 0);
+  lemma_AfterForm(b, asp);
+  Lemma_AlwaysImpliesLaterAlways(asp.synchrony_start, i, eventuallynextwithin(action, span, PaxosTimeMap(b)));
+  reveal eventual();
+  reveal after();
 }
 
 lemma lemma_EstablishRequirementsForWF1RealTime(
-    b:Behavior<RslState>,
-    asp:AssumptionParameters,
-    i:int,
-    action:temporal,
-    span:int
-    )
-    requires LivenessAssumptions(b, asp);
-    requires asp.synchrony_start <= i;
-    requires sat(asp.synchrony_start, always(eventuallynextwithin(action, span, PaxosTimeMap(b))));
-    ensures  sat(i, always(eventuallynextwithin(action, span, PaxosTimeMap(b))));
-    ensures  monotonic_from(i, PaxosTimeMap(b));
+  b:Behavior<RslState>,
+  asp:AssumptionParameters,
+  i:int,
+  action:temporal,
+  span:int
+  )
+  requires LivenessAssumptions(b, asp)
+  requires asp.synchrony_start <= i
+  requires sat(asp.synchrony_start, always(eventuallynextwithin(action, span, PaxosTimeMap(b))))
+  ensures  sat(i, always(eventuallynextwithin(action, span, PaxosTimeMap(b))))
+  ensures  monotonic_from(i, PaxosTimeMap(b))
 {
-    lemma_TimeMonotonicFromInvariantHolds(b, asp, i);
-    Lemma_AlwaysImpliesLaterAlways(asp.synchrony_start, i, eventuallynextwithin(action, span, PaxosTimeMap(b)));
+  lemma_TimeMonotonicFromInvariantHolds(b, asp, i);
+  Lemma_AlwaysImpliesLaterAlways(asp.synchrony_start, i, eventuallynextwithin(action, span, PaxosTimeMap(b)));
 }
     
 
